Mapping to JSCert

coq/JsDefensiveJs.v
@@ -2,10 +2,117 @@ Set Implicit Arguments.
 Require Import Shared.
 Require Import JsSyntax JsSyntaxAux JsCommon JsCommonAux JsPreliminary.
 
-(**************************************************************)
-(** ** Types and Environments for DefensiveJS                 *)
+Require Import LibBag LibFset LibFsetExt LibListExt.
+
+(* ************************************ *)
+(** * Auxiliary tactics                 *)
+
+Ltac false_right := let H := fresh "H" in (try solve [right; introv H; inverts* H]).
+
+
+(* ************************************ *)
+(** * Induction in type                 *)
+
+Lemma peano_induction_type : 
+  forall (P : nat -> Type),
+    (forall n, (forall m, m < n -> P m) -> P n) ->
+    (forall n, P n).
+Proof.
+  introv H. cuts* K: (forall n m, m < n -> P m).
+  induction n; introv Le. 
+
+  destruct m; false; nat_math.
+  apply H. intros. apply IHn. nat_math. 
+Qed.
+
+Lemma measure_induction_type : 
+  forall (A:Type) (mu:A->nat) (P:A->Type),
+    (forall x, (forall y, mu y < mu x -> P y) -> P x) ->
+    (forall x, P x).
+Proof.
+  introv IH. intros x. gen_eq n: (mu x). gen x.
+  induction n using peano_induction_type. introv Eq. subst*.
+Qed.
+
+(* *********************************************************************** *)
+(**  Retrieving information from an indexed list - last occurrence matters *)
+
+Section Φ.
+
+Context (T : Type).
+Context (T_dec : forall (t1 t2 : T), {t1 = t2} + {~ t1 = t2}).
+
+Fixpoint Φ {T : Type} (ρ : list (string * T)) (idx : string) : option T :=
+match ρ with
+ | nil => None
+ | (id, t) :: ρ => let Φρ := Φ ρ idx in
+                   ifb (id = idx) then match Φρ with 
+                                        | None => Some t
+                                        | _    => Φρ
+                                       end
+                                  else Φρ
+end.
+
+Lemma Φ_dec : forall (ρ : list (string * T)) idx oT, {Φ ρ idx = oT} + {~ Φ ρ idx = oT}.
+Proof.
+  induction ρ as [ | (x & τ) ρ]; introv; simpls.
+  + destruct oT; [right | left]; auto; try discriminate. 
+  + destruct (string_dec x idx); cases_if*. 
+    - destruct (Φ ρ idx); jauto.
+      * destruct oT; [ | right; discriminate].
+        destruct ((rm T_dec) t t0) as [Heq | Hneq]; subst; jauto.
+        right; fequals. 
+      * destruct oT; [ | right; discriminate].
+        destruct ((rm T_dec) τ t) as [Heq | Hneq]; subst; jauto.
+        right; fequals. 
+    - rewrite decide_spec in H. apply isTrue_false in n. false*. 
+Qed.
+
+End Φ.
+
+(* ******************************************** *)
+(**  Auxiliary decidability lemmas              *)
+
+Section aux_dec_lemmas.
+
+Context (T : Type).
+Context (T_dec : forall (t1 t2 : T), {t1 = t2} + {~ t1 = t2}).
+
+(* Membership in a list is decidable *)
+Lemma Mem_decidable : forall (t : T) (lT : list T), 
+  {Mem t lT} + {~ Mem t lT}.
+Proof with false_right.
+  inductions lT...
+  inverts IHlT as IHlT. 
+
+  + left; constructor~.
+
+  + specializes T_dec t a. inverts T_dec as T_dec... 
+    left; constructor~.
+Qed.
+
+(* Existence of duplicates in a list is decidable *)
+Lemma noDup_decidable : forall (lT : list T), 
+  {noDup lT} + {~ noDup lT}.
+Proof with false_right.
+  inductions lT.
+  
+  + left; constructor~.
+  + inverts IHlT as IHlT... 
+    lets Hm : (@Mem_decidable a lT). inverts Hm as Hm...
+    left; constructor~.
+Qed.
+
+End aux_dec_lemmas. 
+
+(*************************************************************)
+(** ** Variables and patched finite maps on variables        *)
 
 Definition var := string.
+
+
+(**************************************************************)
+(** ** Types and Environments for DefensiveJS                 *)
 
 (* Types *)
 Inductive τ_main : Type :=
@@ -13,16 +120,16 @@ Inductive τ_main : Type :=
  | τβ : τ_main (* booleans  *)
  | τσ : τ_main (* strings   *)
  | τυ : τ_main (* undefined *)
- | το : (list var * list τ_main) -> τ_main                        (* object   *)
- | τα : τ_main -> nat -> τ_main                                   (* array    *)
- | τϕ : list τ_main -> τ_main -> τ_main                           (* function *)
- | τμ : list τ_main -> list var * list τ_main -> τ_main -> τ_main (* method *)
+ | το : list (var * τ_main) -> τ_main                          (* object   *)
+ | τα : τ_main -> nat -> τ_main                                (* array    *)
+ | τϕ : list τ_main -> τ_main -> τ_main                        (* function *)
+ | τμ : list τ_main -> list (var * τ_main) -> τ_main -> τ_main (* method   *)
 .
 
-Notation "{{ ρ }}"         := (το ρ) (at level 59).
-Notation "[[ τ , n ]]"     := (τα τ n) (at level 59).
-Notation "〈 lτ → τ 〉"     := (τϕ lτ τ) (at level 59).
-Notation "《 lτ [ ρ ] → τ 》" := (τμ lτ ρ τ) (at level 59).
+(* Object types *)
+Definition djs_obj_type := list (var * τ_main).
+
+
 
 (**************************************************************)
 (** ** We have main and auxiliary types. Main types are
@@ -30,7 +137,6 @@ Notation "《 lτ [ ρ ] → τ 》" := (τμ lτ ρ τ) (at level 59).
        are reserved for intermediate terms in pretty-big-step
        style.                 
  *) 
-
 Inductive type : Type :=
  | type_main : τ_main -> type
  | τξ        : type
@@ -38,41 +144,35 @@ Inductive type : Type :=
 
 Coercion type_main : τ_main >-> type.
 
-(* Objects *)
-Definition djs_obj := (list var * list τ_main)%type.
-
-(* Retrieving type of identifier from object *)
-Fixpoint Φ (lx : list var) (lτ : list τ_main) (idx : string) : option τ_main :=
-match lx, lτ with
- | nil, _ => None
- | _, nil => None
- | (id :: lx), (τ :: lτ) => ifb (id = idx) then Some τ
-                                           else Φ lx lτ idx
-end.
+Notation "{{ ρ }}"         := (το ρ) (at level 59).
+Notation "[[ τ , n ]]"     := (τα τ n) (at level 59).
+Notation "〈 lτ → τ 〉"     := (τϕ lτ τ) (at level 59).
+Notation "《 lτ [ ρ ] → τ 》" := (τμ lτ ρ τ) (at level 59).
 
 (* Scope frame kinds *)
 Inductive κ := | κϕ : κ | κω : κ.
 
 (* Typing Environments *)
-Definition typ_env := list (djs_obj * κ).
+Definition typ_env := list (djs_obj_type * κ).  
+
+Notation "∅" := (@nil (djs_obj_type * κ)) (at level 60).
 
 (**************************************************************)
 (** ** Syntactic categories                                   *)
 
 (* Literals *)
 Inductive djs_λ := 
- | djs_η : number -> djs_λ                (* Number  literals *)
- | djs_σ : string -> djs_λ                (* String  literals *)
- | djs_β : bool -> djs_λ                  (* Boolean literals *)
- | djs_α : list djs_ε -> djs_λ            (* Array   literals *)
- | djs_ο : list var * list djs_ε -> djs_λ (* Object  literals *)
+ | djs_η : number -> djs_λ             (* Number  literals *)
+ | djs_σ : string -> djs_λ             (* String  literals *)
+ | djs_β : bool -> djs_λ               (* Boolean literals *)
+ | djs_α : list djs_ε -> djs_λ         (* Array   literals *)
+ | djs_ο : list (var * djs_ε) -> djs_λ (* Object  literals *)
 
 with djs_unop := 
- | djs_unop_to_num  (* Conversion string -> number  *)
- | djs_unop_to_str  (* Conversion number -> string  *)
- | djs_unop_to_bool (* Conversion ______ -> boolean *)
- | djs_unop_min     (* Unary minus *)
- | djs_unop_bin_neg (* Unary binary negation *)
+ | djs_unop_add         (* Conversion string -> number  *)
+ | djs_unop_not         (* Conversion ______ -> boolean *)
+ | djs_unop_neg         (* Unary minus *)
+ | djs_unop_bitwise_neg (* Unary bitwise negation *)
 
 with djs_binop :=
   | djs_binop_add (* + Addition       *)
@@ -126,7 +226,7 @@ with djs_stat :=
 
 (* Functions *)
 with djs_ϕ := 
- | djs_ϕ_main : list (var * τ_main) -> (list var * list djs_δε) -> djs_stat -> djs_ε -> djs_ϕ
+ | djs_ϕ_main : djs_obj_type -> list (var * djs_δε) -> djs_stat -> djs_ε -> djs_ϕ
 
 (* Defined expressions *)
 with djs_δε :=
@@ -140,7 +240,7 @@ with djs_π :=
 (* Intermediate terms *)
 with djs_iterm :=
  | djs_εϕ_aux : list (djs_ε * τ_main) -> djs_iterm
- | djs_ϕ_aux  : list (var * τ_main) -> (list var * list djs_δε) -> djs_stat ->  djs_ε -> djs_obj -> djs_iterm
+ | djs_ϕ_aux  : djs_obj_type -> list (var * djs_δε) -> djs_stat ->  djs_ε -> djs_obj_type -> τ_main -> djs_iterm
 
 (* Terms *)
 with djs_term :=
@@ -163,6 +263,8 @@ Coercion djs_term_δε : djs_δε    >-> djs_term.
 Coercion djs_term_π  : djs_π     >-> djs_term.
 Coercion djs_interm  : djs_iterm >-> djs_term.
 
+Definition djs_obj := list (var * djs_ε).
+
 Implicit Type τ  : τ_main.
 Implicit Type λ  : djs_λ.
 Implicit Type ε  : djs_ε.
@@ -171,7 +273,9 @@ Implicit Type s  : djs_stat.
 Implicit Type ϕ  : djs_ϕ.
 Implicit Type δε : djs_δε.
 Implicit Type π  : djs_π.
-
+Implicit Type ι   : djs_iterm.
+Implicit Type T  : djs_term.
+Implicit Type τρ : djs_obj_type.
 Implicit Type ρ  : djs_obj.
 
 Implicit Type η : number.
@@ -180,49 +284,450 @@ Implicit Type β : bool.
 
 Implicit Type Γ : typ_env.
 
+
+(**************************************************************)
+(** ** Term size                                              *)
+
+Section Sizes.
+
+Open Local Scope nat_scope.
+
+(* Size of main types *)
+Fixpoint djs_size_τ τ :=
+match τ with
+ | τη | τσ | τβ | τυ => 1
+ | τα τ _ => S (djs_size_τ τ) 
+
+ | το τρ => S ((fix djs_size_τρ τρ : nat :=
+              match τρ with 
+               | nil => 1
+               | (_, τ) :: τρ => djs_size_τ τ + djs_size_τρ τρ
+              end) τρ)
+              
+ | τϕ lτ τ => S (((fix djs_size_lτ lτ : nat :=
+                   match lτ with 
+                    | nil => 1
+                    | τ :: lτ => djs_size_τ τ + djs_size_lτ lτ
+                   end) lτ) + djs_size_τ τ)
+
+ | τμ lτ τρ τ => S (((fix djs_size_lτ lτ : nat :=
+                      match lτ with 
+                       | nil => 1
+                       | τ :: lτ => djs_size_τ τ + djs_size_lτ lτ
+                      end) lτ) +
+                    ((fix djs_size_τρ τρ : nat :=
+                      match τρ with 
+                       | nil => 1
+                       | (_, τ) :: τρ => djs_size_τ τ + djs_size_τρ τρ
+                      end) τρ) + djs_size_τ τ)
+end.
+
+(* Size of types *)
+Definition djs_size_type τm :=
+match τm with
+ | type_main τ => djs_size_τ τ
+ | τξ => 1
+end.
+
+(* Size of literals *)
+Fixpoint djs_size_λ λ : nat :=
+match λ with
+ | djs_η _  => 1
+ | djs_σ _  => 1
+ | djs_β _  => 1
+ | djs_α lε => S ((fix djs_size_lε (lε : list djs_ε) : nat :=
+                    match lε with 
+                     | nil => 1
+                     | ε :: lε => djs_size_ε ε + djs_size_lε lε
+                    end) lε)
+ | djs_ο ρ => S ((fix djs_size_ρ ρ : nat :=
+                  match ρ with
+                   | nil => 1
+                   | (_, ε) :: ρ => djs_size_ε ε + djs_size_ρ ρ
+                  end) ρ)
+end 
+
+(* Size of lhs-expressions *)
+with djs_size_λε λε : nat :=
+match λε with
+ | djs_var  _       => 1
+ | djs_prop ε  _    => S (djs_size_ε ε)
+ | djs_cai  ε  _    => S (djs_size_ε ε)
+ | djs_ii   ε1 ε2 _ => S (djs_size_ε ε1 + djs_size_ε ε2)
+ | djs_bai  ε1 ε2   => S (djs_size_ε ε1 + djs_size_ε ε2)
+end
+
+(* Size of expressions *)
+with djs_size_ε ε : nat :=
+match ε with
+ | djs_ε_l     λ       => S (djs_size_λ λ)
+ | djs_ε_λε    λε      => S (djs_size_λε λε)
+ | djs_ε_ass   λε ε    => S (djs_size_λε λε + djs_size_ε ε)
+ | djs_ε_unop  _ ε     => S (djs_size_ε ε)
+ | djs_ε_binop _ ε1 ε2 => S (djs_size_ε ε1 + djs_size_ε ε2)
+ | djs_ε_func  ϕ lε    => S (djs_size_ϕ ϕ + 
+                             ((fix djs_size_lε (lε : list djs_ε) : nat :=
+                               match lε with 
+                                | nil => 1
+                                | ε :: lε => djs_size_ε ε + djs_size_lε lε
+                               end) lε))
+ | djs_csi     ε1 ε2 _ => S (djs_size_ε ε1 + djs_size_ε ε2)
+end
+
+(* Size of statements *)
+with djs_size_stat s :=
+match s with
+ | djs_stat_expr  ε        => S (djs_size_ε ε)
+ | djs_stat_with  ε  s     => S (djs_size_ε ε + djs_size_stat s) 
+ | djs_stat_if    ε  s1 s2 => S (djs_size_ε ε + djs_size_stat s1 + djs_size_stat s2)
+ | djs_stat_while ε  s     => S (djs_size_ε ε + djs_size_stat s) 
+ | djs_stat_seq   ls       => S ((fix djs_size_ls (ls : list djs_stat) : nat :=
+                                  match ls with 
+                                   | nil => 1
+                                   | s :: ls => djs_size_stat s + djs_size_ls ls
+                                  end) ls)
+end
+
+(* Size of functions *)
+with djs_size_ϕ ϕ := 
+match ϕ with
+ | djs_ϕ_main _ lvδε s ε => S (S (((fix djs_size_lvδε lvδε : nat :=
+                                      match lvδε with 
+                                        | nil => 1
+                                        | (_, δε) :: lvδε => djs_size_δε δε + djs_size_lvδε lvδε
+                                      end) lvδε)
+                                  + djs_size_stat s + djs_size_ε ε))
+end
+
+(* Size of defined expressions *)
+with djs_size_δε δε :=
+match δε with
+ | djs_δε_expr ε => S (djs_size_ε ε)
+ | djs_δε_func ϕ => S (djs_size_ϕ ϕ)
+end
+
+(* Size of programs *)
+with djs_size_π π :=
+match π with
+ | djs_π_main ϕ => S (djs_size_ϕ ϕ)
+end
+
+(* Size of intermediate terms *)
+with djs_size_ι ι :=
+match ι with
+ | djs_εϕ_aux lετ => S ((fix djs_size_lετ (lετ : list (djs_ε * τ_main)) : nat :=
+                               match lετ with 
+                                | nil => 1
+                                | (ε, _) :: lετ => djs_size_ε ε + djs_size_lετ lετ
+                               end) lετ)
+
+ | djs_ϕ_aux ly lvδε s ε _ _ => S (((fix djs_size_lvδε lvδε : nat :=
+                                     match lvδε with 
+                                      | nil => 1
+                                      | (_, δε) :: lvδε => djs_size_δε δε + djs_size_lvδε lvδε
+                                            end) lvδε)
+                                      + djs_size_stat s + djs_size_ε ε)
+end
+
+with djs_size_term T :=
+match T with
+ | djs_term_λ  λ  => djs_size_λ λ
+ | djs_term_λε λε => djs_size_λε λε
+ | djs_term_ε  ε  => djs_size_ε  ε
+ | djs_term_s  s  => djs_size_stat s
+ | djs_term_ϕ  ϕ  => djs_size_ϕ ϕ
+ | djs_term_δε δε => djs_size_δε δε
+ | djs_term_π  π  => djs_size_π π
+ | djs_interm  ι   => djs_size_ι ι
+end.
+
+(* Term size is always positive *)
+Lemma djs_size_term_positive : forall T, djs_size_term T > 0.
+Proof.
+  induction T using (measure_induction_type djs_size_term).
+  destruct T; destruct d; simpls; nat_math. 
+Qed.  
+
+End Sizes.
+
+(**************************************************************)
+(** ** Decidability of equality for types and terms            *)
+
+(* Equality of types is decidable *)
+Lemma djs_type_eq_dec : forall (τ1 τ2 : type), {τ1 = τ2} + {τ1 <> τ2}.
+Proof with (false_right; try solve [left; auto]).
+  induction τ1 using (measure_induction_type djs_size_type). 
+
+  destruct τ1; destruct τ2...
+  destruct τ; destruct τ0...
+
+  gen l0; inductions l; destruct l0...
+  destruct a; destruct p; destruct (string_dec v v0)...
+  subst. lets Hτ : X τ τ0. simpls; nat_math.
+  lets Hl : IHl l0. intros. apply X. simpls; nat_math.
+  inverts Hτ as Hτ; try inverts Hτ; inverts Hl as Hl; try inverts Hl...
+
+  lets Hτ : X τ τ0. simpls; nat_math.
+  lets Hn : eq_nat_dec n n0.
+  inverts Hτ as Hτ; try inverts Hτ; inverts Hn...
+
+  lets Hτ : X τ τ0. simpls; nat_math.
+  inverts Hτ as Hτ; try inverts Hτ...
+  gen l0; inductions l; destruct l0...
+  lets Hτ : X a τ. simpls; nat_math.
+  inverts Hτ as Hτ; try inverts Hτ...
+  lets Hl : IHl τ0 l0. intros. apply X. simpls; nat_math.
+  inverts Hl as Hl; try inverts Hl...
+
+  lets Hτ : X τ τ0. simpls; nat_math.
+  inverts Hτ as Hτ; try inverts Hτ...
+  gen l0 l1 l2; inductions l; intros; destruct l1...
+  gen l2; inductions l0; intros; destruct l2...
+  destruct a; destruct p; destruct (string_dec v v0)...
+  subst. lets Hτ : X τ τ1. simpls; nat_math.
+  lets Hl : IHl0 l2. intros. apply X. simpls; nat_math.
+  inverts Hτ as Hτ; try inverts Hτ; inverts Hl as Hl; try inverts Hl...
+  lets Hτ : X a τ. simpls; nat_math.
+  inverts Hτ as Hτ; try inverts Hτ...
+  clear IHl. gen l0 l1 l2; inductions l; intros; destruct l1...
+  gen l2; inductions l0; intros; destruct l2...
+  destruct a; destruct p; destruct (string_dec v v0)...
+  subst. lets Hτ : X τ1 τ2. simpls; nat_math.
+  lets Hl : IHl0 l2. intros. apply X. simpls; nat_math.
+  inverts Hτ as Hτ; try inverts Hτ; inverts Hl as Hl; try inverts Hl...
+  lets Hτ : X a τ1. simpls; nat_math. inverts Hτ as Hτ; try inverts Hτ...
+  lets Hl : IHl τ0 τ l0 l1 l2. intros. apply X. simpls; nat_math.
+  inverts Hl as Hl; try inverts Hl...  
+Qed.
+
+(* Equality on numbers is decidable  *)
+Lemma number_eq_dec : forall n1 n2 : number, {n1 = n2} + {n1 <> n2}.
+Proof with (false_right; auto; try solve [intuition]).
+  inductions n1; destruct n2...
+
+  + destruct b; destruct b0... 
+  + destruct b; destruct b0... 
+  + lets Hm : Pos.eq_dec m m0.
+    lets He : Z.eq_dec e e1.
+    destruct b; destruct b0; intuition; subst... 
+
+    assert (e0 = e2) by (apply proof_irrelevance); subst*.
+    assert (e0 = e2) by (apply proof_irrelevance); subst*.  
+Qed.
+
+(* Equality of terms is decidable *)
+Lemma djs_term_eq_dec : forall (T1 T2 : djs_term), {T1 = T2} + {T1 <> T2}.
+Proof with (false_right; try solve [left; auto]).
+  induction T1 using (measure_induction_type djs_size_term). 
+
+  destruct T1; destruct T2...
+
+  + destruct d; destruct d0...
+    - destruct (number_eq_dec n n0); substs*...
+    - destruct (string_dec s s0); substs*...
+    - destruct b; destruct b0...
+    - cut ({l = l0} + {l <> l0}). 
+      * introv Hyp; destruct Hyp; [substs* | ]...
+      * inductions l; destruct l0...
+        lets Hd : X a d. simpls; nat_math.
+        inverts Hd... inverts H.
+        specializes IHl l0.
+        introv Hs; introv. apply X. 
+        simpls; nat_math.
+        destruct IHl... substs*.
+    - cut ({l = l0} + {l <> l0}). 
+      * introv Hyp; destruct Hyp; [substs* | ]...
+      * inductions l; destruct l0...
+        destruct a; destruct p.
+        destruct (string_dec v v0); substs...
+        lets Hd : X d d0. simpls; nat_math.
+        inverts Hd... inverts H.
+        specializes IHl l0.
+        introv Hs; introv. apply X. 
+        simpls; nat_math.
+        destruct IHl... substs*.
+
+  + destruct d; destruct d0...
+    - destruct (string_dec v v0); substs...
+    - destruct (string_dec v v0); substs...
+      lets H : X d d0; [simpls; nat_math | inverts H; try inverts H0]...
+    - destruct (eq_nat_dec n n0); substs...
+      lets H : X d d0; [simpls; nat_math | inverts H; try inverts H0]...
+    - destruct (eq_nat_dec n n0); substs...
+      lets H : X d d0; [simpls; nat_math | inverts H; try inverts H0]...
+      lets H : X d1 d2; [simpls; nat_math | inverts H; try inverts H0]...
+    - lets H : X d d0; [simpls; nat_math | inverts H; try inverts H0]...
+      lets H : X d1 d2; [simpls; nat_math | inverts H; try inverts H0]...
+  
+  + destruct d; destruct d0...
+    - lets H : X d d0; [simpls; nat_math | inverts H; try inverts H0]...
+    - lets H : X d d0; [simpls; nat_math | inverts H; try inverts H0]...
+    - lets H : X d d0; [simpls; nat_math | inverts H; try inverts H0]...
+      lets H : X d1 d2; [simpls; nat_math | inverts H; try inverts H0]...
+    - lets H : X d1 d2; [simpls; nat_math | inverts H; try inverts H0]...
+      destruct d; destruct d0...
+    - lets H : X d2 d0_1; [simpls; nat_math | inverts H; try inverts H0]...
+      lets H : X d3 d0_2; [simpls; nat_math | inverts H; try inverts H0]...
+      destruct d; destruct d1...
+    - lets H : X d d0; [simpls; nat_math | inverts H; try inverts H0]...
+      cut ({l = l0} + {l <> l0}). 
+      * introv Hyp; destruct Hyp; [substs* | ]...
+      * inductions l; destruct l0...
+        lets Hd : X a d. simpls; nat_math.
+        inverts Hd... inverts H.
+        specializes IHl d0 l0.
+        destruct IHl; substs... 
+        introv Hs; introv. 
+        apply X. simpls; nat_math.
+    - lets H : X d1 d0_1; [simpls; nat_math | inverts H; try inverts H0]...
+      lets H : X d2 d0_2; [simpls; nat_math | inverts H; try inverts H0]...
+      destruct (string_dec s s0); subst...
+  
+  + destruct d; destruct d0...
+    - lets H : X d d0; [simpls; nat_math | inverts H; try inverts H0]...
+    - lets H : X d d0; [simpls; nat_math | inverts H; try inverts H0]...
+      lets H : X d1 d2; [simpls; nat_math | inverts H; try inverts H0]...
+    - lets H : X d1 d; [simpls; nat_math | inverts H; try inverts H0]...
+      lets H : X d2 d0_1; [simpls; nat_math | inverts H; try inverts H0]...
+      lets H : X d3 d0_2; [simpls; nat_math | inverts H; try inverts H0]...
+    - lets H : X d d0; [simpls; nat_math | inverts H; try inverts H0]...
+      lets H : X d1 d2; [simpls; nat_math | inverts H; try inverts H0]...
+    - cut ({l = l0} + {l <> l0}). 
+      * introv Hyp; destruct Hyp; [substs* | ]...
+      * inductions l; destruct l0...
+        lets Hd : X a d. simpls; nat_math.
+        inverts Hd... inverts H.
+        specializes IHl l0. 
+        introv Hs; introv. apply X. 
+        simpls; nat_math.
+        destruct IHl; substs... 
+
+  + destruct d; destruct d0.
+    lets H : X d1 d3; [simpls; nat_math | inverts H; try inverts H0]...
+    lets H : X d2 d4; [simpls; nat_math | inverts H; try inverts H0]...
+    cut ({l = l0} + {l <> l0}). 
+      * introv Hyp; destruct Hyp; [substs* | ]...
+        cut ({d = d0} + {d <> d0}). 
+          introv Hyp; destruct Hyp; [substs* | ]...
+          inductions d; destruct d0...
+          destruct a; destruct p.
+          destruct (string_dec v v0); substs...
+          destruct (djs_type_eq_dec τ τ0); substs... 
+          inverts e. specializes IHd d0 l0 d3 d4.
+          destruct IHd; substs...
+          introv Hs; introv. apply X. 
+          simpls; nat_math.
+      * clear d0. inductions l; destruct l0...
+        destruct a; destruct p.
+        destruct (string_dec v v0); substs...
+        lets H : X d0 d1; substs... 
+        simpls; nat_math.
+        inverts H; try inverts H0...
+        specializes IHl l0 d3 d4.
+        destruct IHl; substs...
+        introv Hs; introv. apply X. 
+        simpls; nat_math.
+  + destruct d; destruct d0...
+    - lets H : X d d0; [simpls; nat_math | inverts H; try inverts H0]...
+    - lets H : X d d0; [simpls; nat_math | inverts H; try inverts H0]...
+
+  + destruct d; destruct d0...
+    lets H : X d d0; [simpls; nat_math | inverts H; try inverts H0]...
+
+  + destruct d; destruct d0...
+    - cut ({l = l0} + {l <> l0}). 
+      * introv Hyp; destruct Hyp; [substs* | ]...
+      * inductions l; destruct l0...
+        destruct a; destruct p.
+        lets H : X d d0; [simpls; nat_math | inverts H; try inverts H0]...
+        destruct (djs_type_eq_dec τ τ0); substs... inverts e. 
+        specializes IHl l0.
+        introv Hs; introv. apply X. 
+        simpls; nat_math.
+        inverts IHl; substs...
+
+    - destruct (djs_type_eq_dec τ τ0); substs... inverts e. 
+      lets H : X d1 d4; [simpls; nat_math | inverts H; try inverts H0]...
+      lets H : X d2 d5; [simpls; nat_math | inverts H; try inverts H0]...
+      assert ({l = l0} + {l <> l0}).
+      {
+        clear - X. inductions l; destruct l0...
+        destruct a; destruct p.
+        destruct (string_dec v v0); substs...
+        lets H : X d0 d1; [simpls; nat_math | inverts H; try inverts H0]...
+        destruct (IHl d3 l0 d4 d5 τ0); substs...
+        introv Hs; apply X; simpls; nat_math.
+      }
+      assert ({d = d0} + {d <> d0}).
+      {
+        clear - X. inductions d; destruct d0...
+        destruct a; destruct p.
+        destruct (string_dec v v0); substs...
+        destruct (djs_type_eq_dec τ τ1); substs... inverts e.
+        destruct (IHd l d3 d0 d4 d5 τ0); substs...
+        introv Hs; apply X; simpls; nat_math.
+      }
+      assert ({d3 = d6} + {d3 <> d6}).
+      {
+        clear - X. inductions d3; destruct d6...
+        destruct a; destruct p.
+        destruct (string_dec v v0); substs...
+        destruct (djs_type_eq_dec τ τ1); substs... inverts e.
+        destruct (IHd3 d4 d5 d6 τ0); substs...
+        introv Hs; apply X; simpls; nat_math.
+      } intuition; subst...
+Qed.
+
+
 (**************************************************************)
 (** ** Typing                                                 *)
 
-Notation "∅" := (@nil (djs_obj * κ)) (at level 60).
+Section Typing.
 
 Reserved Notation "Γ |- Τ ∷ τ" (at level 60).
 
 Inductive types : typ_env -> djs_term -> type -> Prop := 
 
  (* Literals *)
- | typing_Num    : forall η, ∅ |- (djs_η η) ∷ τη 
- | typing_String : forall σ, ∅ |- (djs_σ σ) ∷ τσ
- | typing_Bool   : forall β, ∅ |- (djs_β β) ∷ τβ
+ | typing_Num    : forall Γ η, Γ |- (djs_η η) ∷ τη 
+ | typing_String : forall Γ σ, Γ |- (djs_σ σ) ∷ τσ
+ | typing_Bool   : forall Γ β, Γ |- (djs_β β) ∷ τβ
 
- | typing_Array_cn : forall ε τ, 
-                       ∅ |- ε ∷ τ -> 
-                       ∅ |- (djs_α (ε :: nil)) ∷ [[τ, 1]]
+ | typing_Array_cn : forall ε τ Γ, 
+                       Γ |- ε ∷ τ -> 
+                       Γ |- (djs_α (ε :: nil)) ∷ [[τ, 1]]
 
- | typing_Array_cc : forall ε1 ε2 lε τ n,
-                       ∅ |- ε1 ∷ τ -> 
-                       ∅ |- djs_α (ε2 :: lε) ∷ [[τ, n]] -> 
-                       ∅ |- (djs_α (ε1 :: ε2 :: lε)) ∷ [[τ, S n]]
+ | typing_Array_cc : forall ε1 τ Γ ε2 lε n,
+                       Γ |- ε1 ∷ τ -> 
+                       Γ |- djs_α (ε2 :: lε) ∷ [[τ, n]] -> 
+                       Γ |- (djs_α (ε1 :: ε2 :: lε)) ∷ [[τ, S n]]
 
- | typing_Object_nil : ∅ |- djs_ο (nil, nil) ∷ {{ (nil, nil) }}
+ | typing_Object_nil : forall Γ, Γ |- djs_ο nil ∷ {{ nil }}
 
- | typing_Object_cons : forall x ε τ lε lτ lx,
-                          ∅ |- ε ∷ τ ->
-                          ∅ |- djs_ο (lx, lε) ∷ {{ (lx, lτ) }} ->
-                          ∅ |- djs_ο ((x :: lx), (ε :: lε)) ∷ {{ ((x :: lx), (τ :: lτ)) }}
+ (* 
+    Requirement : no variable can be equal to "this"
+    Choice      : variables cannot be duplicated
+ *)
+ | typing_Object_cons : forall x ε τ Γ τρ ρ, 
+                            x <> "this" ->
+                            Γ |- ε ∷ τ ->
+                            Γ |- (djs_ο ρ) ∷ {{ τρ }} ->
+                            Γ |- djs_ο ((x, ε) :: ρ) ∷ {{ (x, τ) :: τρ }}
 
  (* Left-hand-side expressions *)
- | typing_VarLoc : forall Γ lx lε x τ, 
-                     Φ lx lε x = Some τ ->
-                     (((lx, lε), κω) :: Γ) |- djs_term_λε (djs_var x) ∷ τ
+ | typing_VarLoc : forall Γ τρ x τ κ, 
+                     Φ τρ x = Some τ ->
+                     ((τρ, κ) :: Γ) |- djs_term_λε (djs_var x) ∷ τ
 
- | typing_VarFS  : forall Γ ρ x lx lε τ, 
-                     Mem x lx -> Γ |- (djs_var x) ∷ τ -> 
-                     (((lx, lε), κϕ) :: Γ) |- (djs_var x) ∷ τ
+ | typing_VarFS  : forall Γ τρ x τ,
+                     let lx := fst (split τρ) in
+                     ~ Mem x lx -> Γ |- (djs_var x) ∷ τ -> 
+                       ((τρ, κϕ) :: Γ) |- (djs_var x) ∷ τ
 
- | typing_Prop : forall Γ ε lx lτ, 
-                   Γ |- ε ∷ (το (lx, lτ)) -> 
+ | typing_Prop : forall Γ ε τρ, 
+                   Γ |- ε ∷ (το τρ) -> 
                    forall x τ, 
-                     Mem (x, τ) (combine lx lτ) ->
+                     Φ τρ x = Some τ ->
                      Γ |- (djs_prop ε x) ∷ τ
 
  | typing_CAI : forall Γ ε m (η : nat) τ, 
@@ -251,85 +756,115 @@ Inductive types : typ_env -> djs_term -> type -> Prop :=
                   Γ |- (djs_ε_λε λε) ∷ τ
 
  (* Casts to number from string, string from number, and anything to bool *)
- | typing_NumCast  : forall Γ ε  , Γ |- ε ∷ τσ -> Γ |- (djs_ε_unop djs_unop_to_num  ε) ∷ τη
- | typing_StrCast  : forall Γ ε  , Γ |- ε ∷ τη -> Γ |- (djs_ε_unop djs_unop_to_str  ε) ∷ τσ
- | typing_BoolCast : forall Γ ε τ, Γ |- ε ∷ τ  -> Γ |- (djs_ε_unop djs_unop_to_bool ε) ∷ τβ
+ | typing_NumCast  : forall Γ ε  , Γ |- ε ∷ τσ -> Γ |- (djs_ε_unop djs_unop_add ε) ∷ τη
+ | typing_BoolCast : forall Γ ε τ, Γ |- ε ∷ τ  -> Γ |- (djs_ε_unop djs_unop_not ε) ∷ τβ
 
  (* Concatenation of strings *)
- | typing_Concat : forall Γ ε1 ε2, Γ |- ε1 ∷ τσ -> Γ |- ε2 ∷ τσ -> 
-                                   Γ |- (djs_ε_binop djs_binop_add ε1 ε2) ∷ τσ
+ | typing_Concat : forall Γ ε1 ε2, 
+     Γ |- ε1 ∷ τσ -> Γ |- ε2 ∷ τσ -> 
+     Γ |- (djs_ε_binop djs_binop_add ε1 ε2) ∷ τσ
 
  (* Unary minus and bit-by-bit negation *)
- | typing_Unary_min :     forall Γ ε, Γ |- ε ∷ τη -> Γ |- (djs_ε_unop djs_unop_min     ε) ∷ τη
- | typing_Unary_bin_neg : forall Γ ε, Γ |- ε ∷ τη -> Γ |- (djs_ε_unop djs_unop_bin_neg ε) ∷ τη
+ | typing_Unary_min :     forall Γ ε, Γ |- ε ∷ τη -> Γ |- (djs_ε_unop djs_unop_neg         ε) ∷ τη
+ | typing_Unary_bin_neg : forall Γ ε, Γ |- ε ∷ τη -> Γ |- (djs_ε_unop djs_unop_bitwise_neg ε) ∷ τη
 
  (* Arithmetic operators +, -, *, /, % *)
- | typing_Arith_add : forall Γ ε1 ε2, Γ |- ε1 ∷ τη -> Γ |- ε1 ∷ τη ->
-                                      Γ |- (djs_ε_binop djs_binop_add ε1 ε2) ∷ τη
- | typing_Arith_sub : forall Γ ε1 ε2, Γ |- ε1 ∷ τη -> Γ |- ε1 ∷ τη ->
-                                      Γ |- (djs_ε_binop djs_binop_sub ε1 ε2) ∷ τη
- | typing_Arith_mul : forall Γ ε1 ε2, Γ |- ε1 ∷ τη -> Γ |- ε1 ∷ τη ->
-                                      Γ |- (djs_ε_binop djs_binop_mul ε1 ε2) ∷ τη
- | typing_Arith_div : forall Γ ε1 ε2, Γ |- ε1 ∷ τη -> Γ |- ε1 ∷ τη ->
-                                      Γ |- (djs_ε_binop djs_binop_div ε1 ε2) ∷ τη
- | typing_Arith_mod : forall Γ ε1 ε2, Γ |- ε1 ∷ τη -> Γ |- ε1 ∷ τη ->
-                                      Γ |- (djs_ε_binop djs_binop_mod ε1 ε2) ∷ τη
+ | typing_Arith_add : forall Γ ε1 ε2, 
+                        Γ |- ε1 ∷ τη -> Γ |- ε2 ∷ τη ->
+                         Γ |- (djs_ε_binop djs_binop_add ε1 ε2) ∷ τη
+ | typing_Arith_sub : forall Γ ε1 ε2, 
+                        Γ |- ε1 ∷ τη -> Γ |- ε2 ∷ τη ->
+                        Γ |- (djs_ε_binop djs_binop_sub ε1 ε2) ∷ τη
+ | typing_Arith_mul : forall Γ ε1 ε2, 
+                        Γ |- ε1 ∷ τη -> Γ |- ε2 ∷ τη ->
+                        Γ |- (djs_ε_binop djs_binop_mul ε1 ε2) ∷ τη
+ | typing_Arith_div : forall Γ ε1 ε2, 
+                        Γ |- ε1 ∷ τη -> Γ |- ε2 ∷ τη ->
+                        Γ |- (djs_ε_binop djs_binop_div ε1 ε2) ∷ τη
+ | typing_Arith_mod : forall Γ ε1 ε2, 
+                        Γ |- ε1 ∷ τη -> Γ |- ε2 ∷ τη ->
+                        Γ |- (djs_ε_binop djs_binop_mod ε1 ε2) ∷ τη
+ | typing_Arith_str : forall Γ ε1, 
+                        Γ |- ε1 ∷ τη -> 
+                        Γ |- (djs_ε_binop djs_binop_add ε1 (djs_ε_l (djs_σ ""))) ∷ τσ
 
  (* Arithmetic bit-operators |, &, ^ *)
- | typing_Arith_bit_or  : forall Γ ε1 ε2, Γ |- ε1 ∷ τη -> Γ |- ε1 ∷ τη ->
-                                          Γ |- (djs_ε_binop djs_binop_bor  ε1 ε2) ∷ τη
- | typing_Arith_bit_and : forall Γ ε1 ε2, Γ |- ε1 ∷ τη -> Γ |- ε1 ∷ τη ->
-                                          Γ |- (djs_ε_binop djs_binop_band ε1 ε2) ∷ τη
- | typing_Arith_bit_xor : forall Γ ε1 ε2, Γ |- ε1 ∷ τη -> Γ |- ε1 ∷ τη ->
-                                          Γ |- (djs_ε_binop djs_binop_bxor ε1 ε2) ∷ τη
+ | typing_Arith_bit_or  : forall Γ ε1 ε2, 
+     Γ |- ε1 ∷ τη -> Γ |- ε2 ∷ τη ->
+     Γ |- (djs_ε_binop djs_binop_bor  ε1 ε2) ∷ τη
+ | typing_Arith_bit_and : forall Γ ε1 ε2, 
+     Γ |- ε1 ∷ τη -> Γ |- ε2 ∷ τη ->
+     Γ |- (djs_ε_binop djs_binop_band ε1 ε2) ∷ τη
+ | typing_Arith_bit_xor : forall Γ ε1 ε2, 
+     Γ |- ε1 ∷ τη -> Γ |- ε2 ∷ τη ->
+     Γ |- (djs_ε_binop djs_binop_bxor ε1 ε2) ∷ τη
 
  (* Arithmetic shift-operators <<, >>, >>> *)
- | typing_Arith_lsh  : forall Γ ε1 ε2, Γ |- ε1 ∷ τη -> Γ |- ε1 ∷ τη ->
-                                       Γ |- (djs_ε_binop djs_binop_lsh ε1 ε2) ∷ τη
- | typing_Arith_rsh  : forall Γ ε1 ε2, Γ |- ε1 ∷ τη -> Γ |- ε1 ∷ τη ->
-                                       Γ |- (djs_ε_binop djs_binop_rsh ε1 ε2) ∷ τη
- | typing_Arith_ursh : forall Γ ε1 ε2, Γ |- ε1 ∷ τη -> Γ |- ε1 ∷ τη ->
-                                       Γ |- (djs_ε_binop djs_binop_ursh ε1 ε2) ∷ τη
+ | typing_Arith_lsh  : forall Γ ε1 ε2, 
+                         Γ |- ε1 ∷ τη -> Γ |- ε2 ∷ τη ->
+                         Γ |- (djs_ε_binop djs_binop_lsh ε1 ε2) ∷ τη
+ | typing_Arith_rsh  : forall Γ ε1 ε2, 
+                         Γ |- ε1 ∷ τη -> Γ |- ε2 ∷ τη ->
+                         Γ |- (djs_ε_binop djs_binop_rsh ε1 ε2) ∷ τη
+ | typing_Arith_ursh : forall Γ ε1 ε2,
+                         Γ |- ε1 ∷ τη -> Γ |- ε2 ∷ τη ->
+                         Γ |- (djs_ε_binop djs_binop_ursh ε1 ε2) ∷ τη
 
  (* Comparisons for numbers: >=, <=, >, <, ==, != *)
- | typing_Comp_ν_gt  : forall Γ ε1 ε2, Γ |- ε1 ∷ τη -> Γ |- ε1 ∷ τη ->
-                                       Γ |- (djs_ε_binop djs_binop_gt ε1 ε2) ∷ τη
- | typing_Comp_ν_lt  : forall Γ ε1 ε2, Γ |- ε1 ∷ τη -> Γ |- ε1 ∷ τη ->
-                                       Γ |- (djs_ε_binop djs_binop_lt ε1 ε2) ∷ τη
- | typing_Comp_ν_ge  : forall Γ ε1 ε2, Γ |- ε1 ∷ τη -> Γ |- ε1 ∷ τη ->
-                                       Γ |- (djs_ε_binop djs_binop_ge ε1 ε2) ∷ τη
- | typing_Comp_ν_le  : forall Γ ε1 ε2, Γ |- ε1 ∷ τη -> Γ |- ε1 ∷ τη ->
-                                       Γ |- (djs_ε_binop djs_binop_le ε1 ε2) ∷ τη
- | typing_Comp_ν_eq  : forall Γ ε1 ε2, Γ |- ε1 ∷ τη -> Γ |- ε1 ∷ τη ->
-                                       Γ |- (djs_ε_binop djs_binop_eq ε1 ε2) ∷ τη
- | typing_Comp_ν_neq : forall Γ ε1 ε2, Γ |- ε1 ∷ τη -> Γ |- ε1 ∷ τη ->
-                                       Γ |- (djs_ε_binop djs_binop_neq ε1 ε2) ∷ τη
+ | typing_Comp_ν_gt  : forall Γ ε1 ε2, 
+                         Γ |- ε1 ∷ τη -> Γ |- ε2 ∷ τη ->
+                         Γ |- (djs_ε_binop djs_binop_gt ε1 ε2) ∷ τη
+ | typing_Comp_ν_lt  : forall Γ ε1 ε2, 
+                         Γ |- ε1 ∷ τη -> Γ |- ε2 ∷ τη ->
+                         Γ |- (djs_ε_binop djs_binop_lt ε1 ε2) ∷ τη
+ | typing_Comp_ν_ge  : forall Γ ε1 ε2, 
+                         Γ |- ε1 ∷ τη -> Γ |- ε2 ∷ τη ->
+                         Γ |- (djs_ε_binop djs_binop_ge ε1 ε2) ∷ τη
+ | typing_Comp_ν_le  : forall Γ ε1 ε2, 
+                         Γ |- ε1 ∷ τη -> Γ |- ε2 ∷ τη ->
+                         Γ |- (djs_ε_binop djs_binop_le ε1 ε2) ∷ τη
+ | typing_Comp_ν_eq  : forall Γ ε1 ε2, 
+                         Γ |- ε1 ∷ τη -> Γ |- ε2 ∷ τη ->
+                         Γ |- (djs_ε_binop djs_binop_eq ε1 ε2) ∷ τη
+ | typing_Comp_ν_neq : forall Γ ε1 ε2, 
+                         Γ |- ε1 ∷ τη -> Γ |- ε2 ∷ τη ->
+                         Γ |- (djs_ε_binop djs_binop_neq ε1 ε2) ∷ τη
 
  (* Comparisons for strings: >=, <=, >, <, ==, != *)
- | typing_Comp_σ_gt  : forall Γ ε1 ε2, Γ |- ε1 ∷ τσ -> Γ |- ε1 ∷ τσ ->
-                                       Γ |- (djs_ε_binop djs_binop_gt ε1 ε2) ∷ τσ
- | typing_Comp_σ_lt  : forall Γ ε1 ε2, Γ |- ε1 ∷ τσ -> Γ |- ε1 ∷ τσ ->
-                                       Γ |- (djs_ε_binop djs_binop_lt ε1 ε2) ∷ τσ
- | typing_Comp_σ_ge  : forall Γ ε1 ε2, Γ |- ε1 ∷ τσ -> Γ |- ε1 ∷ τσ ->
-                                       Γ |- (djs_ε_binop djs_binop_ge ε1 ε2) ∷ τσ
- | typing_Comp_σ_le  : forall Γ ε1 ε2, Γ |- ε1 ∷ τσ -> Γ |- ε1 ∷ τσ ->
-                                       Γ |- (djs_ε_binop djs_binop_le ε1 ε2) ∷ τσ
- | typing_Comp_σ_eq  : forall Γ ε1 ε2, Γ |- ε1 ∷ τσ -> Γ |- ε1 ∷ τσ ->
-                                       Γ |- (djs_ε_binop djs_binop_eq ε1 ε2) ∷ τσ
- | typing_Comp_σ_neq : forall Γ ε1 ε2, Γ |- ε1 ∷ τσ -> Γ |- ε1 ∷ τσ ->
-                                       Γ |- (djs_ε_binop djs_binop_neq ε1 ε2) ∷ τσ
+ | typing_Comp_σ_gt  : forall Γ ε1 ε2, 
+                         Γ |- ε1 ∷ τσ -> Γ |- ε2 ∷ τσ ->
+                         Γ |- (djs_ε_binop djs_binop_gt ε1 ε2) ∷ τσ
+ | typing_Comp_σ_lt  : forall Γ ε1 ε2, 
+                         Γ |- ε1 ∷ τσ -> Γ |- ε2 ∷ τσ ->
+                         Γ |- (djs_ε_binop djs_binop_lt ε1 ε2) ∷ τσ
+ | typing_Comp_σ_ge  : forall Γ ε1 ε2, 
+                         Γ |- ε1 ∷ τσ -> Γ |- ε2 ∷ τσ ->
+                         Γ |- (djs_ε_binop djs_binop_ge ε1 ε2) ∷ τσ
+ | typing_Comp_σ_le  : forall Γ ε1 ε2, 
+                         Γ |- ε1 ∷ τσ -> Γ |- ε2 ∷ τσ ->
+                         Γ |- (djs_ε_binop djs_binop_le ε1 ε2) ∷ τσ
+ | typing_Comp_σ_eq  : forall Γ ε1 ε2, 
+                         Γ |- ε1 ∷ τσ -> Γ |- ε2 ∷ τσ ->
+                         Γ |- (djs_ε_binop djs_binop_eq ε1 ε2) ∷ τσ
+ | typing_Comp_σ_neq : forall Γ ε1 ε2, 
+                         Γ |- ε1 ∷ τσ -> Γ |- ε2 ∷ τσ ->
+                         Γ |- (djs_ε_binop djs_binop_neq ε1 ε2) ∷ τσ
 
- (* Comparisons for numbers: ==, != *)
- | typing_Comp_β_eq  : forall Γ ε1 ε2, Γ |- ε1 ∷ τβ -> Γ |- ε1 ∷ τβ ->
-                                       Γ |- (djs_ε_binop djs_binop_eq ε1 ε2) ∷ τβ
- | typing_Comp_β_neq : forall Γ ε1 ε2, Γ |- ε1 ∷ τβ -> Γ |- ε1 ∷ τβ ->
-                                       Γ |- (djs_ε_binop djs_binop_neq ε1 ε2) ∷ τβ
+ (* Comparisons for booleans: ==, != *)
+ | typing_Comp_β_eq  : forall Γ ε1 ε2, 
+                         Γ |- ε1 ∷ τβ -> Γ |- ε2 ∷ τβ ->
+                         Γ |- (djs_ε_binop djs_binop_eq ε1 ε2) ∷ τβ
+ | typing_Comp_β_neq : forall Γ ε1 ε2, 
+                         Γ |- ε1 ∷ τβ -> Γ |- ε2 ∷ τβ ->
+                         Γ |- (djs_ε_binop djs_binop_neq ε1 ε2) ∷ τβ
 
  (* Operators for booleans: ||, && *)
- | typing_Bool_or  : forall Γ ε1 ε2, Γ |- ε1 ∷ τβ -> Γ |- ε1 ∷ τβ ->
-                                     Γ |- (djs_ε_binop djs_binop_or  ε1 ε2) ∷ τβ
- | typing_Bool_and : forall Γ ε1 ε2, Γ |- ε1 ∷ τβ -> Γ |- ε1 ∷ τβ ->
-                                     Γ |- (djs_ε_binop djs_binop_and ε1 ε2) ∷ τβ
+ | typing_Bool_or  : forall Γ ε1 ε2, 
+                       Γ |- ε1 ∷ τβ -> Γ |- ε2 ∷ τβ ->
+                       Γ |- (djs_ε_binop djs_binop_or  ε1 ε2) ∷ τβ
+ | typing_Bool_and : forall Γ ε1 ε2, 
+                       Γ |- ε1 ∷ τβ -> Γ |- ε2 ∷ τβ ->
+                       Γ |- (djs_ε_binop djs_binop_and ε1 ε2) ∷ τβ
 
  (* Assignment *)
  | typing_Assign : forall Γ λε ε τ, 
@@ -344,7 +879,8 @@ Inductive types : typ_env -> djs_term -> type -> Prop :=
                            Γ |- (djs_ε_func ϕ lε) ∷ τ
 
  
- | typing_FunctionCall_aux_nil : forall Γ, Γ |- djs_εϕ_aux nil ∷ τξ
+ | typing_FunctionCall_aux_nil : forall Γ, 
+                                   Γ |- djs_εϕ_aux nil ∷ τξ
 
  | typing_FunctionCall_aux_cons : forall Γ ε τ lετ,
                                     Γ |- ε ∷ τ ->
@@ -358,18 +894,24 @@ Inductive types : typ_env -> djs_term -> type -> Prop :=
                   Γ |- (djs_csi ε ε' σ) ∷ τσ
 
  (* Expressions are statements *)
- | typing_Expression : forall Γ ε τ, Γ |- ε ∷ τ -> Γ |- (djs_stat_expr ε) ∷ τυ
+ | typing_Expression : forall Γ ε τ, 
+                         Γ |- ε ∷ τ -> Γ |- (djs_stat_expr ε) ∷ τυ
 
  (* With statement *)
- | typing_With : forall Γ ε s ρ, Γ |- ε ∷ (το ρ) -> ((ρ, κω) :: Γ) |- s ∷ τυ ->
-                                 Γ |- (djs_stat_with ε s) ∷ τυ
+ | typing_With : forall Γ ε s τρ, 
+                   Γ |- ε ∷ (το τρ) -> ((τρ, κω) :: Γ) |- s ∷ τυ ->
+                   Γ |- (djs_stat_with ε s) ∷ τυ
 
  (* If-then-else statement *)
- | typing_If : forall Γ ε s1 s2, Γ |- ε ∷ τβ -> Γ |- s1 ∷ τυ -> Γ |- s2 ∷ τυ ->
-                                 Γ |- (djs_stat_if ε s1 s2) ∷ τυ
+ | typing_If : forall Γ ε s1 s2, 
+                 Γ |- ε ∷ τβ -> Γ |- s1 ∷ τυ -> Γ |- s2 ∷ τυ ->
+                 Γ |- (djs_stat_if ε s1 s2) ∷ τυ
+
  (* While statement *)
- | typing_While : forall Γ ε s, Γ |- ε ∷ τβ -> Γ |- s ∷ τυ ->
-                                  Γ |- (djs_stat_while ε s) ∷ τυ
+ | typing_While : forall Γ ε s,
+                    Γ |- ε ∷ τβ -> Γ |- s ∷ τυ ->
+                    Γ |- (djs_stat_while ε s) ∷ τυ
+
  (* A sequence of statements *)
  | typing_Sequence_nil : forall Γ, Γ |- djs_stat_seq nil ∷ τυ
 
@@ -382,36 +924,63 @@ Inductive types : typ_env -> djs_term -> type -> Prop :=
     Function definition
 
     IMPORTANT: Currently, types for x_i variables must be provided.
-
     TODO: Can/should we infer the types for x_i somehow?
+
+    Strict mode requirement : x_i variables cannot contain duplicates
+    Requirement : no x_i except the first can be equal to "this"
+    Requirement : no y_i can be equal to "this"
+
+    Choice : y_i variables cannot contain duplicates
+    Choice : x_i and y_i must be disjoint
+
+    There may be no free occurrences of 'this' in the body
  *)
+ | typing_FunctionDef_main : forall Γ τρx (τρy : list (var * djs_δε)) ls ε τr, 
+     let lx := fst (split τρx) in
+     let lτ := snd (split τρx) in
+     let ly := fst (split τρy) in
+     let lδε := snd (split τρy) in
+     noDup lx -> noDup ly ->
+     Forall (fun x => x <> "this") lx ->
+     Forall (fun y => y <> "this") ly ->
+     disjoint (from_list lx) (from_list ly) ->
+     Γ |- (djs_ϕ_aux τρx τρy (djs_stat_seq ls) ε nil τr) ∷ τξ ->
+     Γ |- (djs_ϕ_main τρx τρy (djs_stat_seq ls) ε) ∷ 〈 lτ → τr 〉
 
  (* Base case *)
-| typing_FunctionDef_main : forall Γ lxτ ly ls ε lτ τr,
-    Γ |- (djs_ϕ_aux  lxτ ly (djs_stat_seq ls) ε (nil, nil)) ∷ τξ ->
-    Γ |- (djs_ϕ_main lxτ ly (djs_stat_seq ls) ε)            ∷ 〈 lτ → τr 〉
-
-
- (* Base case *)
- | typing_FunctionDef_nil : forall Γ lxτ ε ls τr lx' lτ',
-     let lx := fst (split lxτ) in
-     let lτ := snd (split lxτ) in
-     (((lx ++ lx', lτ ++ lτ')%list, κϕ) :: Γ) |- (djs_stat_seq ls) ∷ τυ ->
-     (((lx ++ lx', lτ ++ lτ')%list, κϕ) :: Γ) |- ε ∷ τr ->
-     Γ  |- (djs_ϕ_aux lxτ (nil, nil) (djs_stat_seq ls) ε (lx', lτ')) ∷ τξ
+ | typing_FunctionDef_nil : forall Γ τρx ε ls τρ τ,
+     (((τρx ++ τρ)%list, κϕ) :: Γ) |- (djs_stat_seq ls) ∷ τυ ->
+     (((τρx ++ τρ)%list, κϕ) :: Γ) |- ε ∷ τ ->
+     Γ  |- (djs_ϕ_aux τρx nil (djs_stat_seq ls) ε τρ τ) ∷ τξ
 
  (* Recursive call *)
- | typing_FunctionDef_cons : forall Γ lxτ ε τ y ly δε lδε ls lx' lτ',
-     let lx := fst (split lxτ) in
-     let lτ := snd (split lxτ) in
-     (((lx ++ lx', lτ ++ lτ')%list, κϕ) :: Γ) |- δε ∷ τ ->
-     Γ |- djs_ϕ_aux lxτ (ly, lδε) (djs_stat_seq ls) ε (lx' & y, lτ' & τ) ∷ τξ ->
-     Γ |- djs_ϕ_aux lxτ (y :: ly, δε :: lδε) (djs_stat_seq ls) ε (lx', lτ') ∷ τξ
+ | typing_FunctionDef_cons : forall Γ τρx τρy ε τ y δε ls τρ τ',
+     (((τρx ++ τρ)%list, κϕ) :: Γ) |- δε ∷ τ ->
+     Γ |- djs_ϕ_aux τρx τρy (djs_stat_seq ls) ε (τρ & (y, τ)) τ' ∷ τξ ->
+     Γ |- djs_ϕ_aux τρx ((y, δε) :: τρy) (djs_stat_seq ls) ε τρ τ' ∷ τξ
 
-(* Method definition *)
- | typing_MethodDef : forall Γ lxτ ρy ls ε lτ ρ τ,
-     Γ |- (djs_ϕ_main (("this", {{ ρ }}) :: lxτ) ρy (djs_stat_seq ls) ε) ∷ 〈 ({{ ρ }} :: lτ) → τ 〉->
-     Γ |- (djs_ϕ_main lxτ ρy (djs_stat_seq ls) ε) ∷ 《 lτ [ρ] → τ 》
+(* 
+    Method definition
+
+    Strict mode requirement : x_i variables cannot contain duplicates
+    Requirement : no x_i except the first can be equal to "this"
+
+    Choice : y_i variables cannot contain duplicates
+    Choice : x_i and y_i must be disjoint
+
+    There need to be free occurrences of 'this' in the body
+ *)
+ | typing_MethodDef : forall Γ τρx τρy ls ε τρ τr,
+     let lx  := fst (split τρx) in
+     let lτ  := snd (split τρx) in
+     let ly  := fst (split τρy) in
+     let lδε := snd (split τρy) in
+     noDup lx -> noDup ly ->
+     Forall (fun x => x <> "this") lx ->
+     Forall (fun y => y <> "this") ly ->
+     disjoint (from_list lx) (from_list ly) ->
+     Γ |- (djs_ϕ_aux (("this", {{ τρ }}) :: τρx) τρy (djs_stat_seq ls) ε nil τr) ∷ τξ ->
+     Γ |- (djs_ϕ_main τρx τρy (djs_stat_seq ls) ε) ∷ 《 lτ [τρ] → τr 》
 
  (* Defined expressions *)
  | typing_DefExprExpr : forall Γ ε τ, Γ |- ε ∷ τ -> Γ |- (djs_δε_expr ε) ∷ τ
@@ -423,6 +992,651 @@ Inductive types : typ_env -> djs_term -> type -> Prop :=
 
 where "Γ |- T ∷ τ" := (types Γ T τ).
 
+(* ********************************************************** *)
+(** * Auxiliary inversion lemmas *)
+
+(* Weakening only from the left *)
+Lemma weakening_from_left : forall T (τ : type) Γ, 
+  (Γ |- T ∷ τ -> forall Γ', (Γ ++ Γ')%list |- T ∷ τ).
+Proof.
+  induction T using (measure_induction djs_size_term); introv HD;
+  destruct T as [λ | λε | ε | s | ϕ | δε | π | ι]; destruct τ; introv; inversion HD; substs*;
+  try solve [constructor; try applys* H; simpls; nat_math];
+  try solve [econstructor; try eassumption; try applys* H; simpls; nat_math].
+
+  + constructor~; applys* H;
+    lets Hsize : djs_size_term_positive ε1;
+    simpls; nat_math.
+
+  + constructor~; applys* H;
+    lets Hsize : djs_size_term_positive ε;
+    simpls; nat_math.
+  
+  + rewrite app_cons. applys~ typing_VarFS.
+    clear - H4. inductions Γ0. inverts H4.
+    destruct a. inversion H4; substs; rewrite app_cons.
+    constructor~. applys~ typing_VarFS.
+
+  + apply typing_Arith_str. applys* H.
+    simpls; nat_math.
+
+  + econstructor; try eassumption; applys* H; [simpls; nat_math | ].
+    clear - H4. inductions lε; lets Hsize : djs_size_term_positive ϕ.
+    - simpls; nat_math.
+    - simpls. destruct lτ; [false* | ].
+      assert (length lε = length lτ) by (rew_length in *; nat_math).
+      specializes IHlε H; nat_math.
+
+  + econstructor; try eassumption. applys* H. simpls; nat_math.
+    specializes H H4. simpls; nat_math. eapply H.
+
+  + econstructor; try eassumption; applys* H; [simpls; nat_math | ].
+    lets Hsize : djs_size_term_positive s0. 
+    simpls; nat_math.
+
+  + econstructor; applys* H; [simpls; nat_math | ].
+    lets Hsize : djs_size_term_positive ε. 
+    simpls; nat_math.
+
+  + constructor; rewrite <- app_cons; applys* H; simpls; nat_math.
+
+  + econstructor; [ | applys* H]. 
+    - rewrite <- app_cons; applys* H. simpls; nat_math.
+    - lets Hsize : djs_size_term_positive δε. 
+      simpls; nat_math.
+Qed.
+
+(* Weakening from empty context *)
+Lemma weakening_empty : forall T (τ : type), 
+  ∅ |- T ∷ τ -> forall Γ, Γ |- T ∷ τ.
+Proof.
+  introv HD; introv.
+  apply weakening_from_left with (Γ' := Γ) in HD; auto.
+Qed.
+
+(* Strengthening *)
+Lemma strengthening : forall T (τ : type) Γ τρ Γ',
+  ((Γ & (τρ, κω)) ++ Γ')%list |- T ∷ τ -> (Γ & (τρ, κω)) |- T ∷ τ.
+Proof.
+  induction T using (measure_induction djs_size_term); introv HD;
+  destruct T as [λ | λε | ε | s | ϕ | δε | π | ι]; destruct τ; introv; inversion HD; substs*;
+  try solve [constructor; try applys* H; simpls; nat_math];
+  try solve [econstructor; try eassumption; try applys* H; simpls; nat_math].
+
+  + constructor~; applys* H;
+    lets Hsize : djs_size_term_positive ε1;
+    simpls; nat_math.
+
+  + constructor~; applys* H;
+    lets Hsize : djs_size_term_positive ε;
+    simpls; nat_math.
+  
+  + destruct Γ.
+    - rewrite app_last_sym in *. rewrite app_nil_l in *. 
+      inverts H0. applys~ typing_VarLoc.
+    - rewrite app_last_sym in *. rewrite app_cons in *.
+      inverts H0. applys~ typing_VarLoc.
+
+  + destruct Γ; rewrite app_last_sym in *. 
+    - rewrite app_nil_l in *. inverts H0. 
+    - rewrite app_cons in *. inverts H0. 
+      rewrite <- app_last_sym in H4. 
+      applys~ typing_VarFS.
+
+      clear - H4. gen τ; inductions Γ; introv Hyp; rewrite app_last_sym in *.
+      * rewrite app_nil_l in *. inverts Hyp. constructor~.
+      * destruct a as (τρa & κa). rewrite app_cons in *. inversion Hyp; substs.
+        constructor~. rewrite <- app_last_sym in H5. applys~ typing_VarFS. applys* IHΓ.
+
+  + apply typing_Arith_str. applys* H.
+    simpls; nat_math.
+
+  + econstructor; try eassumption; applys* H; [simpls; nat_math | ].
+    clear - H4. inductions lε; lets Hsize : djs_size_term_positive ϕ.
+    - simpls; nat_math.
+    - simpls. destruct lτ; [false* | ].
+      assert (length lε = length lτ) by (rew_length in *; nat_math).
+      specializes IHlε H; nat_math.
+
+  + econstructor; try eassumption. applys* H. simpls; nat_math.
+    repeat rewrite <- app_cons in H4. 
+    specializes H H4. simpls; nat_math. eapply H.
+
+  + econstructor; try eassumption; applys* H; [simpls; nat_math | ].
+    lets Hsize : djs_size_term_positive s0. 
+    simpls; nat_math.
+
+  + econstructor; applys* H; [simpls; nat_math | ].
+    lets Hsize : djs_size_term_positive ε. 
+    simpls; nat_math.
+
+  + constructor; repeat rewrite <- app_cons in *; applys* H; simpls; nat_math.
+
+  + econstructor; [ | applys* H]. 
+    - rewrite <- app_cons in *; applys* H; simpls; nat_math.
+    - lets Hsize : djs_size_term_positive δε. 
+      simpls; nat_math.
+Qed.
+
+(* Array length correctness *)
+Lemma array_length : forall Γ lε τ n, Γ |- djs_α lε ∷ [[τ, n]] -> n = length lε.
+Proof.
+  introv Hr. inductions Hr; 
+  [ | specializes IHHr2 (ε2 :: lε0) τ n0 (@eq_refl djs_term) (@eq_refl type)];
+  rew_length in *; nat_math.
+Qed.
+
+(* All elements of an array are of the same type *)
+Lemma array_same_type : forall Γ lε τ n, Γ |- djs_α lε ∷ [[τ, n]] -> Forall (fun ε => Γ |- ε ∷ τ) lε.
+Proof with (repeat constructor*).
+  inductions lε; introv HD; inverts HD; repeat constructor*.
+Qed.
+
+(* All statements are of type 'undefined' *)
+Lemma statement_undefined : forall Γ s τ, Γ |- s ∷ τ -> τ = τυ.
+Proof.
+  introv HD; inverts~ HD.
+Qed.
+
+Lemma same_variables_in_objects : forall ρ τρ Γ,
+  Γ |- djs_ο ρ ∷ {{τρ}} -> fst (split ρ) = fst (split τρ).
+Proof.
+  inductions ρ; introv HD; simpls; [inverts~ HD | ].
+  destruct τρ; [inverts~ HD | ].
+  inverts HD. specializes IHρ H6.
+  rewrite (split_combine_fs ρ). rewrite combine_split; 
+  [ | rewrite split_length_l; rewrite~ split_length_r].
+  rewrite (split_combine_fs τρ); simpls; rewrite combine_split;
+  [ | rewrite split_length_l; rewrite~ split_length_r]; simpls*.
+  rewrite~ IHρ.
+Qed.
+    
+(****************************************************************)
+(** ** Translation to JSCert                                    *)
+
+Definition toJSC_unop (u : djs_unop) :=
+match u with
+ | djs_unop_add => unary_op_add (* Conversion to number *)
+ | djs_unop_not => unary_op_not (* Conversion to boolean AND negation *) 
+ | djs_unop_neg => unary_op_neg (* Unary minus *)
+ | djs_unop_bitwise_neg => unary_op_bitwise_not (* Bitwise negation *)
+end.
+
+Definition toJSC_binop (b : djs_binop) :=
+match b with
+  | djs_binop_add => binary_op_add  (* + Addition       *)
+  | djs_binop_sub => binary_op_sub  (* - Subtraction    *)
+  | djs_binop_mul => binary_op_mult (* * Multiplication *)
+  | djs_binop_div => binary_op_div  (* / Division       *)
+  | djs_binop_mod => binary_op_mod  (* % Modulus        *)
+
+  | djs_binop_band => binary_op_bitwise_and          (* &   Bitwise and          *)
+  | djs_binop_bor  => binary_op_bitwise_or           (* |   Bitwise or           *)
+  | djs_binop_bxor => binary_op_bitwise_xor          (* ^   Bitwise xor          *)
+  | djs_binop_lsh  => binary_op_left_shift           (* <<  Shift left           *)
+  | djs_binop_rsh  => binary_op_right_shift          (* >>  Shift right          *)
+  | djs_binop_ursh => binary_op_unsigned_right_shift (* >>> Unsigned shift right *)
+
+  | djs_binop_and => binary_op_and (* && Boolean and *)
+  | djs_binop_or  => binary_op_or  (* || Boolean or  *)
+
+  | djs_binop_eq  => binary_op_equal    (* == Equality   *)
+  | djs_binop_neq => binary_op_disequal (* != Inequality *)
+  | djs_binop_gt  => binary_op_gt       (* >  *)
+  | djs_binop_lt  => binary_op_lt       (* <  *)
+  | djs_binop_ge  => binary_op_ge       (* >= *)
+  | djs_binop_le  => binary_op_le       (* <= *)
+end.
+
+Fixpoint toJSC_λ (λ : djs_λ) :=
+match λ with
+ | djs_η n  => expr_literal (literal_number n) 
+ | djs_σ s  => expr_literal (literal_string s) 
+ | djs_β b  => expr_literal (literal_bool   b)
+ | djs_α lε => expr_array   ((fix toJSC_lε (lε : list djs_ε) :=
+                               match lε with 
+                                | nil => nil
+                                | ε :: lε => (Some (toJSC_ε ε)) :: toJSC_lε lε
+                               end) lε)   
+ | djs_ο ρ  => expr_object  ((fix toJSC_ρ (ρ : djs_obj) :=
+                                match ρ with
+                                  | nil => nil
+                                  | (x, ε) :: ρ => (propname_identifier x, propbody_val (toJSC_ε ε)) :: toJSC_ρ ρ
+                                end) ρ)     
+end
+
+with toJSC_λε λε := 
+match λε with
+ | djs_var  x => expr_identifier x                  
+ | djs_prop ε x => expr_member (toJSC_ε ε) x           
+
+ | djs_cai  ε n => expr_access (toJSC_ε ε) 
+                               (expr_literal (literal_number (JsNumber.of_int n)))
+
+ | djs_ii   ε1 ε2 n => expr_access (toJSC_ε ε1)
+                                   (expr_binary_op
+                                      (toJSC_ε ε2)
+                                      binary_op_bitwise_and
+                                      (expr_literal (literal_number (JsNumber.of_int n))))
+
+ | djs_bai  ε1 ε2 => let JSCε1 := toJSC_ε ε1 in
+                     let JSCε2 := toJSC_ε ε2 in
+                       expr_access JSCε1 
+                                   (expr_binary_op 
+                                      (expr_binary_op
+                                         JSCε2
+                                         binary_op_unsigned_right_shift
+                                         (expr_literal (literal_number JsNumber.zero)))
+                                       binary_op_mod
+                                       (expr_member JSCε1 "length"))
+end
+
+with toJSC_ε ε := 
+match ε with 
+ | djs_ε_l     λ => toJSC_λ λ
+ | djs_ε_λε    λε => toJSC_λε λε
+ | djs_ε_ass   λε ε => expr_assign (toJSC_λε λε) None (toJSC_ε ε)
+ | djs_ε_unop  unop ε => expr_unary_op (toJSC_unop unop) (toJSC_ε ε)
+ | djs_ε_binop binop ε1 ε2 => expr_binary_op (toJSC_ε ε1) (toJSC_binop binop) (toJSC_ε ε2)
+
+ | djs_csi     ε1 ε2 σ => let JSCε1 := toJSC_ε ε1 in
+                          let JSCε2rsh0 := (expr_binary_op 
+                                              (toJSC_ε ε2)
+                                              binary_op_unsigned_right_shift
+                                              (expr_literal (literal_number JsNumber.zero))) in
+                            expr_conditional 
+                              (expr_binary_op 
+                                 JSCε2rsh0
+                                 binary_op_lt
+                                 (expr_member JSCε1 "length"))
+                              (expr_access JSCε1 JSCε2rsh0)
+                              (expr_literal (literal_string σ))
+
+ | djs_ε_func ϕ lε => expr_call 
+                        (toJSC_ϕ ϕ)
+                        ((fix toJSC_lε lε :=
+                            match lε with
+                             | nil => nil
+                             | ε :: lε => (toJSC_ε ε) :: toJSC_lε lε
+                            end
+                         ) lε)
+end
+
+with toJSC_stat s := 
+match s with
+ | djs_stat_expr  ε        => stat_expr (toJSC_ε ε)
+ | djs_stat_with  ε  s     => stat_with (toJSC_ε ε) (toJSC_stat s)
+ | djs_stat_if    ε  s1 s2 => stat_if (toJSC_ε ε) (toJSC_stat s1) (Some (toJSC_stat s2))
+ | djs_stat_while ε  s     => stat_while nil (toJSC_ε ε) (toJSC_stat s)
+ | djs_stat_seq   ls       => stat_block ((fix toJSC_lstat ls := 
+                                            match ls with
+                                             | nil => nil
+                                             | s :: ls => (toJSC_stat s) :: (toJSC_lstat ls)
+                                            end) ls)
+end
+
+(* Functions *)
+with toJSC_ϕ ϕ := 
+match ϕ with
+ | djs_ϕ_main τρx τρy s ε => 
+     let lx := fst (split τρx) in
+       expr_function 
+         None (* Functions have no names *)
+         lx   (* List of variables       *)
+         (* Function body *)
+         (funcbody_intro 
+            (prog_intro 
+               true (* Body is always strict *)
+               (
+                 (* Variables *) element_stat (stat_var_decl 
+                                                 ((fix var_decl τρy :=
+                                                     match τρy with
+                                                       | nil => nil
+                                                       | (y, δε) :: τρy => (y, Some (toJSC_δε δε)) :: var_decl τρy
+                                                     end) τρy)) ::
+                 (* Statement *) element_stat (toJSC_stat s) :: 
+                 (* Return    *) element_stat (stat_return (Some (toJSC_ε ε))) :: nil
+               )
+            )
+            "function() {}"
+         )                                                                                         
+end
+
+(* Defined expressions *)
+with toJSC_δε δε :=
+match δε with
+ | djs_δε_expr ε => toJSC_ε ε
+ | djs_δε_func ϕ => toJSC_ϕ ϕ
+end
+
+(* Programs *)
+with toJSC_π π :=
+match π with
+ | djs_π_main ϕ => let JSCϕ := (toJSC_ϕ ϕ) in
+                   prog_intro 
+                     true
+                     (
+                       element_stat (stat_var_decl (("_", Some JSCϕ) :: nil)) ::
+                       element_stat (stat_return 
+                                       (Some (expr_function None ("x" :: nil)
+                                               (funcbody_intro
+                                                  (prog_intro 
+                                                     true
+                                                     (
+                                                       element_stat (stat_if (expr_binary_op
+                                                                                (expr_unary_op
+                                                                                   unary_op_typeof
+                                                                                   (expr_identifier "x")
+                                                                                )
+                                                                                binary_op_equal 
+                                                                                (expr_literal (literal_string "string"))
+                                                                             ) 
+                                                                             (stat_return (Some (expr_call 
+                                                                                                   JSCϕ
+                                                                                                   (expr_identifier "x" :: nil))))
+                                                                             None)
+                                                       :: nil
+                                                     )                                                     
+                                                  ) 
+                                                  "function() {}"
+                                               )
+                                             )
+                                       )
+                                    )
+                       :: nil
+                     )
+end.
+
+(*
+Lemma djs_unicity_of_types_λε : 
+  forall λε Γ τm1 τm2 
+         (IH : forall T : djs_term,
+                 lt (djs_size_term T) (djs_size_term λε) ->
+                  forall Γ (τm1 τm2 : type), Γ |- T ∷ τm1 -> Γ |- T ∷ τm2 -> τm1 = τm2),
+    Γ |- λε ∷ τm1 -> Γ |- λε ∷ τm2 -> τm1 = τm2.
+Proof.
+  introv IH HD1 HD2; destruct λε; try solve [inverts HD1; inverts~ HD2].
+
+  + induction Γ; [inverts HD1 | ].
+    destruct a. destruct κ0; inverts HD1; inverts* HD2.    
+    rewrite H6 in H4. inverts~ H4.
+
+  + inverts HD1; inverts HD2.
+    lets Hτ : IH H3 H2. simpls; nat_math. inverts Hτ.
+    lets Hnd : no_duplicates_in_objects H3.
+    clear -H4 H6 Hnd. gen τ τ0 v. 
+    inductions τρ; intros; [inverts H4 | ]. destruct a. 
+    rewrite (split_combine_fs τρ) in *. repeat (rewrite combine_split in *; 
+    [ | rewrite split_length_l; rewrite~ split_length_r]; simpls).
+    inverts* H4. inverts~ H6. 
+    eapply mem_comb in H0; [ | rewrite split_length_l; rewrite~ split_length_r]; false*.
+    inverts* H6. eapply mem_comb in H0; [ | rewrite split_length_l; rewrite~ split_length_r]; false*.
+
+  + inverts HD1; inverts HD2.
+    lets Hτ : IH H2 H3. simpls; nat_math. inverts~ Hτ.
+
+  + inverts HD1; inverts HD2.
+    lets Hτ : IH H2 H3. simpls; nat_math. inverts~ Hτ.
+
+  + inverts HD1; inverts HD2.
+    lets Hτ : IH H2 H3. simpls; nat_math. inverts~ Hτ.
+Qed.
+
+Lemma djs_unicity_of_types : forall T Γ τm1 τm2,
+  Γ |- T ∷ τm1 -> Γ |- T ∷ τm2 -> τm1 = τm2.
+Proof.
+  induction T using (measure_induction djs_size_term).
+  destruct T as [λ | λε | ε | s | ϕ | δε | π | ι]; introv HD1 HD2.
+
+  + eapply djs_unicity_of_types_λ; jauto. 
+  + eapply djs_unicity_of_types_λε; jauto. 
+  + admit.
+  + inverts HD1; inverts~ HD2.
+  + inversion HD1; inversion HD2; substs; inverts H9;
+    subst lx ly lx0 ly0 lτ lτ0 lδε lδε0; substs; tryfalse.
+    
+    - cut (τr = τr0); [intro Hyp; substs~ | ]. 
+      cut (exists Γ, Γ |- ε ∷ τr /\ Γ |- ε ∷ τr0).
+      * introv (Γ0 & (HD1' & HD2')). 
+        specializes H HD1' HD2'; [ | inverts~ H].
+        lets Hsize : djs_size_term_positive ε; simpls; rew_length; nat_math.
+      * {
+          cut (Forall (fun δε => forall Γ τm1 τm2, Γ |- δε ∷ τm1 -> Γ |- δε ∷ τm2 -> τm1 = τm2) (snd (split τρy))). 
+          + clear - H7 H16.
+            remember nil as τρ. clear Heqτρ.
+            gen Γ τρ τr τr0. inductions τρy; intros.
+            - inverts H7. inverts H16. eexists; jauto.
+            - destruct a. inverts H7. inverts H16.
+              rewrite (split_combine_fs _) in H. rewrite combine_split in *; 
+              [ | rewrite split_length_l; rewrite~ split_length_r]; simpls.
+              rewrite (split_combine_fs _) in H. rewrite combine_split in *; 
+              [ | rewrite split_length_l; rewrite~ split_length_r]; simpls.
+              inverts H. specializes H2 H3 H4. inverts H2.              
+              eapply IHτρy; eassumption.
+          + rewrite <- Forall_Mem; introv Hm.
+            apply H. clear - Hm.
+            gen ls ε. inductions τρy; intros. inverts Hm.
+            destruct a. rewrite (split_combine_fs _) in Hm. rewrite combine_split in *; 
+            [ | rewrite split_length_l; rewrite~ split_length_r]; simpls.
+            rewrite (split_combine_fs _) in Hm. rewrite combine_split in *; 
+            [ | rewrite split_length_l; rewrite~ split_length_r]; simpls.
+            inverts Hm as Hm. nat_math. specializes IHτρy Hm ls ε. nat_math.         
+        }
+
+    - cut (τr = τr0 /\ τρ = τρ0); [intros (Hyp1 & Hyp2); substs~ | ]. 
+      clear H2 H3 H4 H5 HD1 H13 H10 H11 H12 HD2 H14.
+
+      cut (exists Γ, Γ |- ε ∷ τr /\ Γ |- ε ∷ τr0).
+      * introv (Γ0 & (HD1' & HD2')). 
+        specializes H HD1' HD2'; [ | inverts~ H].
+        lets Hsize : djs_size_term_positive ε; simpls; rew_length; nat_math.
+      * {
+          cut (Forall (fun δε => forall Γ τm1 τm2, Γ |- δε ∷ τm1 -> Γ |- δε ∷ τm2 -> τm1 = τm2) (snd (split τρy))). 
+          + clear - H7 H16.
+            remember nil as τρ. clear Heqτρ.
+            gen Γ τρ τr τr0. inductions τρy; intros.
+            - inverts H7. inverts H16. eexists; jauto.
+            - destruct a. inverts H7. inverts H16.
+              rewrite (split_combine_fs _) in H. rewrite combine_split in *; 
+              [ | rewrite split_length_l; rewrite~ split_length_r]; simpls.
+              rewrite (split_combine_fs _) in H. rewrite combine_split in *; 
+              [ | rewrite split_length_l; rewrite~ split_length_r]; simpls.
+              inverts H. specializes H2 H3 H4. inverts H2.              
+              eapply IHτρy; eassumption.
+          + rewrite <- Forall_Mem; introv Hm.
+            apply H. clear - Hm.
+            gen ls ε. inductions τρy; intros. inverts Hm.
+            destruct a. rewrite (split_combine_fs _) in Hm. rewrite combine_split in *; 
+            [ | rewrite split_length_l; rewrite~ split_length_r]; simpls.
+            rewrite (split_combine_fs _) in Hm. rewrite combine_split in *; 
+            [ | rewrite split_length_l; rewrite~ split_length_r]; simpls.
+            inverts Hm as Hm. nat_math. specializes IHτρy Hm ls ε. nat_math.         
+        }
+
+        admit.
+
+    - subst lx lτ ly lτ0. inverts H8.
+      
+
+  + inverts HD1; inverts~ HD2; eapply H; try eassumption;
+    simpls; nat_math.
+  + inverts HD1; inverts~ HD2.
+  + inverts HD1; inverts~ HD2.
+Qed. 
+
+Lemma djs_type_inference_λ : 
+  forall λ Γ (IH : forall T, djs_size_term T < djs_size_λ λ ->
+    { τm | Γ |- T ∷ τm } + {forall (τm : type), ~ Γ |- T ∷ τm }), 
+    { τm | Γ |- λ ∷ τm } + {forall (τm : type), ~ Γ |- λ ∷ τm }.
+Proof with (try solve [right; introv NoNo; inverts* NoNo]).
+  intros; destruct λ as [η | σ | β | lε | ρ]; destruct Γ...
+
+  + left; exists τη. constructor.
+  + left; exists τσ. constructor.
+  + left; exists τβ. constructor.
+
+  + destruct lε as [ | ε1 lε]...
+    destruct lε as [ | ε2 lε].
+
+    - destruct (IH ε1) as [(τm & Hε1) | ]... simpls; nat_math.
+      destruct τm as [τ | ]; [ | false; inverts Hε1]... 
+      left; eexists. constructor*.
+
+    - destruct (IH ε1) as [(τm & Hε1) | ]... simpls; nat_math.
+      destruct τm as [τ | ]; [ | false; inverts Hε1]... 
+      
+      destruct (IH (djs_α (ε2 :: lε))) as [(τm & Hε2) | ]...
+      lets Hsize : djs_size_term_positive ε1; simpls; rew_length; nat_math.
+      destruct τm as [τ' | ]; [ | false; inverts Hε2]...       
+      destruct (IH ε2) as [(τm & Hε2') | ]... simpls; nat_math.
+      destruct τm as [τ'' | ]; [ | false; inverts Hε2']...
+      destruct (djs_type_eq_dec τ'' τ).
+      * inverts e... destruct τ'; try solve [false; inverts Hε2].
+        lets Heq : array_length Hε2; subst.
+        destruct (djs_type_eq_dec τ' τ).
+          inverts e. left; eexists; constructor; eassumption.
+          false. inverts Hε2. simpls.
+Qed.
+
+Lemma DJS_Type_Inference : forall T Γ (τm : type), 
+  {exists (τm : type), Γ |- T ∷ τm} + {~ exists (τm : type), Γ |- T ∷ τm}.
+Proof.
+  induction T using (measure_induction_type djs_size_term).
+
+  destruct T as [λ | λε | ε | s | ϕ | δε | π | ι]; simpls.
+
+  
+  
+  + intros; destruct λ as [η | σ | β | lε | ρ].
+Qed. 
+
+Lemma DJS_Typing_Decidable : forall T Γ (τm : type), {Γ |- T ∷ τm} + {~ Γ |- T ∷ τm}.
+Proof with false_right.
+  intro T. induction T using (measure_induction_type djs_size_term).
+
+  destruct T as [λ | λε | ε | s | ϕ | δε | π | ι]; simpls.
+
+Lemma aux_typ_dec_λ : 
+  forall λ Γ (τm : type) 
+         (IH : forall T, djs_size_term T < djs_size_λ λ ->
+                 forall Γ (τm : type), {Γ |- T ∷ τm} + {~ Γ |- T ∷ τm}), 
+    {Γ |- λ ∷ τm} + {~ Γ |- λ ∷ τm}.
+Proof with false_right.
+  intros; destruct λ as [η | σ | β | lε | ρ]; 
+  destruct Γ; false_right; destruct τm; try destruct τ; false_right;
+  try solve [left; constructor].
+
+  + destruct lε as [ | ε1 lε]...
+    destruct lε as [ | ε2 lε]. 
+
+    - lets Hε : IH ε1 (∅) τ. simpls; nat_math.      
+      inverts Hε as Hε... 
+      lets Hn : eq_nat_dec n 1. inverts Hn as Hn;
+      [ | right; introv Hyp; apply array_length in Hyp; rew_length in *; nat_math].
+      left; constructor~.
+
+    - lets Hn : eq_nat_dec n (length (ε1 :: ε2 :: lε)). inverts Hn as Hn;
+      [ | right; introv Hyp; apply array_length in Hyp; rew_length in *; nat_math].
+      lets Hε : IH ε1 (∅) τ. simpls; nat_math.
+      inverts Hε as Hε...
+      replace (length (ε1 :: ε2 :: lε)) with (S (length (ε2 :: lε))) by (rew_length; nat_math).
+      lets Hlε : IH (djs_α (ε2 :: lε)) (∅) ([[τ, length (ε2 :: lε)]]). 
+      lets Hsize : djs_size_term_positive ε1. simpls; rew_length; nat_math.
+      inverts Hlε as Hlε... left; constructor~.
+
+  + destruct ρ as [ | xε ρ]; destruct l...
+
+    - left; constructor~. 
+
+    - destruct xε as (x & ε). destruct p as (x' & τε).
+      lets Hx : string_dec x' x. inverts Hx as Hx... 
+      lets Hρl : IH (djs_ο ρ) (∅) ({{l}}). 
+      lets Hsize : djs_size_term_positive ε. simpls; rew_length; nat_math. 
+      inverts Hρl as Hρl...
+      lets Hε : IH ε (∅) τε. simpls; nat_math. 
+      inverts Hε as Hε...
+      lets Hx : string_dec x "this". inverts Hx as Hx... 
+      lets HD : (@noDup_decidable _ (x :: fst (split ρ)) string_dec).
+      inverts HD as HD. left; constructor~.
+      right; introv Hyp; inversion Hyp; substs; subst lx; auto.
+Qed.
+
+Lemma aux_typ_dec_λε : 
+  forall λε Γ (τm : type) 
+         (IH : forall T, djs_size_term T < djs_size_λε λε ->
+                 forall Γ (τm : type), {Γ |- T ∷ τm} + {~ Γ |- T ∷ τm}), 
+    {Γ |- λε ∷ τm} + {~ Γ |- λε ∷ τm}.
+Proof with false_right.
+  intros; destruct λε as [x | ε x | ε η | ε1 ε2 η | ε1 ε2];
+  try destruct τ...
+
+  + admit.
+
+  + admit.
+
+  + destruct Γ; [ | right; introv Hyp; inverts Hyp as Hyp; inverts Hyp]; 
+    try destruct τm... 
+
+Lemma aux_typ_dec_ε_α : forall ε τ (τm : type) 
+         (IH : forall T, djs_size_term T < djs_size_ε ε ->
+                 forall Γ (τm : type), {Γ |- T ∷ τm} + {~ Γ |- T ∷ τm}), 
+    {exists m, ∅ |- ε ∷ [[τ, m]]} + {~ exists m, ∅ |- ε ∷ [[τ, m]]}.
+Proof with (try solve [right; introv (m & Hyp); inverts Hyp as Hyp; inverts* Hyp]).
+  destruct ε as [λ | λε | | | | |].
+
+  + destruct λ as [ | | | lε |]...
+    destruct lε as [ | ε1 lε]...
+    destruct lε as [ | ε2 lε].
+    
+    - lets Hε : IH ε1 (∅) τ. simpls; nat_math.      
+      inverts Hε as Hε... 
+      left. exists 1. repeat constructor~. 
+
+    - 
+Qed.
+
+  + admit.
+
+  + admit.
+Qed.
+
+| typing_Prop : forall Γ ε τρ, 
+                   Γ |- ε ∷ (το τρ) -> 
+                   forall x τ, 
+                     Mem (x, τ) τρ ->
+                     Γ |- (djs_prop ε x) ∷ τ
+
+ | typing_CAI : forall Γ ε m (η : nat) τ, 
+                Γ |- ε ∷ (τα τ m) -> 
+                η < m ->
+                Γ |- (djs_cai ε η) ∷ τ
+
+ | typing_II : forall Γ ε ε' τ m (η : nat), 
+                 Γ |- ε  ∷ (τα τ m) ->
+                 Γ |- ε' ∷ τη -> η < m -> (m <= 1073741824)%Z ->
+                 Γ |- (djs_ii ε ε' η) ∷ τ
+
+ | typing_BAI : forall Γ (ε ε' : djs_ε) τ m, 
+                  Γ |- ε  ∷ (τα τ m) ->
+                  Γ |- ε' ∷ τη -> 
+                  Γ |- (djs_bai ε ε') ∷ τ
+
+
+(* PROOOOOF *)
+
+  (* Literals *)
+  + intros; applys~ aux_typ_dec_λ.
+
+  + .
+
+  + destruct .
+
+  + admit.
+
+  + admit.
+
+  + destruct δε as [ε | ϕ]; apply X; simpls. rew_length. nat_math.
+
 (**************************************************************)
 (** ** Lemmas for arrays                                      *)
 
@@ -432,28 +1646,12 @@ Proof.
   introv Hr. inverts Hr; nat_math. 
 Qed.
 
-(* All ellements of an array are of the same type *)
-Lemma array_same_type : forall Γ lε τ n, Γ |- djs_α lε ∷ [[τ, n]] -> Forall (fun ε => Γ |- ε ∷ τ) lε.
-Proof with (repeat constructor*).
-  inductions lε; introv HD; inverts HD; repeat constructor*.
-Qed.
 
-(* Array length correctness *)
-Lemma array_length : forall Γ lε τ n, Γ |- djs_α lε ∷ [[τ, n]] -> n = length lε.
-Proof.
-  introv Hr. inductions Hr; 
-  [ |   specializes IHHr2 (ε2 :: lε0) τ n0 (@eq_refl djs_term) (@eq_refl type)];
-  rew_length in *; nat_math.
-Qed.
 
 (**************************************************************)
 (** ** Lemmas for statements                                  *)
 
-(* All statements are of type 'undefined' *)
-Lemma statement_undefined : forall Γ s τ, Γ |- s ∷ τ -> τ = τυ.
-Proof.
-  introv HD; inverts~ HD.
-Qed.
+
 
 (**************************************************************)
 (** ** Lemmas for functions                                   *)
@@ -498,10 +1696,466 @@ Lemma untypable_object : forall Γ τ,
   -> False. 
 Proof.
   introv HD. 
-    inverts HD as HD. inverts H7. 
-    inverts HD as HD. clear H6. destruct lτ. clear H5.
-    inverts HD. inversion H1. simpls. substs. subst lx lτ.
+    inverts HD. clear H5 H6. inverts H8. 
+    inverts H7 as HD. clear H6. destruct lτ. clear H5.
+    inverts HD. clear H6 H7 H8 H9. 
+    inversion H10. simpls. substs. subst lx0 lτ.
     repeat rewrite app_nil_l in *.
-    inverts H7. inverts H2. inverts H4.
+    inverts H6. inverts H1. inverts H3.
     rew_length in H5; nat_math.
 Qed.     
+
+(* Typing objects *)
+Lemma objects_typable_only_from_empty : 
+  forall Γ lπ τ, Γ |- djs_ο lπ ∷ τ -> Γ = ∅.
+Proof.
+  introv HD. inverts~ HD. 
+Qed.
+
+(* No typable object contains a "this" variable *)
+Lemma objects_no_this : 
+  forall Γ lπ τ, Γ |- djs_ο lπ ∷ τ -> ~ Mem "this" (fst lπ). 
+Proof.
+  introv HD. inductions HD; introv Hm; inverts* Hm. 
+Qed.
+
+
+
+
+
+
+
+
+
+
+
+
+
+
+
+
+
+
+
+
+(**************************************************************)
+(** ** Detecting unbound this's                               
+
+Section has_this.
+
+(*
+   Numbers, strings, and booleans do not have a 'this'.
+
+   An array has a 'this' if any of its elements has a 'this'
+
+   An object has a this if there exists a 'this' in one of the expressions
+*)
+Fixpoint has_this_λ λ :=
+match λ with 
+ | djs_η _ | djs_σ _ | djs_β _ => False
+ | djs_α lε => ((fix has_this_lε (lε : list djs_ε) : Prop :=
+                   match lε with 
+                     | nil => False
+                     | ε :: lε => has_this_ε ε \/ has_this_lε lε
+                   end) lε)
+ | djs_ο ρ => ((fix has_this_ρ ρ : Prop :=
+                  match ρ with 
+                    | nil => False
+                    | (_, ε) :: ρ => has_this_ε ε \/ has_this_ρ ρ
+                  end) ρ)
+end
+
+(*
+   'this' in expressions is fully recursive
+*)
+with has_this_ε ε := 
+match ε with 
+ | djs_ε_l     λ        => has_this_λ  λ
+ | djs_ε_λε    λε       => has_this_λε λε
+ | djs_ε_ass   λε ε     => has_this_λε λε \/ has_this_ε ε
+ | djs_ε_unop  _  ε     => has_this_ε ε
+ | djs_ε_binop _  ε1 ε2 => has_this_ε ε1 \/ has_this_ε ε2
+ | djs_ε_func  ϕ  lε    => has_this_ϕ ϕ \/ 
+                           ((fix has_this_lε (lε : list djs_ε) : Prop :=
+                               match lε with 
+                                 | nil => False
+                                 | ε :: lε => has_this_ε ε \/ has_this_lε lε
+                               end) lε)
+ | djs_csi     ε1 ε2 _  => has_this_ε ε1 \/ has_this_ε ε2
+end
+
+(*
+   For lhs-expressions:
+
+   A variable has a 'this' if it is 'this'
+
+   'this' can never occur as a property in a typable lhs-expression
+*)
+with has_this_λε λε := 
+match λε with
+ | djs_var  x       => (x = "this")
+ | djs_prop ε  _    => has_this_ε ε
+ | djs_cai  ε  _    => has_this_ε ε
+ | djs_ii   ε1 ε2 _ => has_this_ε ε1 \/ has_this_ε ε2
+ | djs_bai  ε1 ε2   => has_this_ε ε1 \/ has_this_ε ε2
+end
+
+(*
+   'this' in statements is fully recursive
+*)
+with has_this_stat s :=
+match s with
+ | djs_stat_expr  ε         => has_this_ε ε
+ | djs_stat_with  ε  s      => has_this_ε ε \/ has_this_stat s
+ | djs_stat_if    ε  s1 s2  => has_this_ε ε \/ has_this_stat s1 \/ has_this_stat s2
+ | djs_stat_while ε  s1     => has_this_ε ε \/ has_this_stat s1
+ | djs_stat_seq   ls        => ((fix has_this_ls (ls : list djs_stat) : Prop :=
+                                   match ls with 
+                                     | nil => False
+                                     | s :: ls => has_this_stat s \/ has_this_ls ls
+                                   end) ls)
+end
+
+(*
+   'this' in defined expressions is fully recursive
+*)
+with has_this_δε δε :=
+match δε with 
+ | djs_δε_expr ε => has_this_ε ε
+ | djs_δε_func ϕ => has_this_ϕ ϕ
+end
+
+(*
+   Functions have a 'this' if 
+     the first parameter is not 'this' and
+     the body has a 'this'
+*)
+with has_this_ϕ ϕ := 
+match ϕ with 
+ | djs_ϕ_main τρ lvδε s ε => match τρ with
+                               | (x, _) :: _ => ifb (x = "this") then False
+                                                else (((fix has_this_lvδε lvδε :=
+                                                          match lvδε with 
+                                                            | nil => False
+                                                            | (_, δε) :: lvδε => has_this_δε δε \/ has_this_lvδε lvδε
+                                                          end) lvδε)
+                                                      \/ has_this_stat s \/ has_this_ε ε)   
+                               | _ => (((fix has_this_lvδε lvδε :=
+                                           match lvδε with 
+                                             | nil => False
+                                             | (_, δε) :: lvδε => has_this_δε δε \/ has_this_lvδε lvδε
+                                           end) lvδε)
+                                       \/ has_this_stat s \/ has_this_ε ε)
+                             end
+end.
+
+(*
+   'this' in programs is fully recursive
+*)
+Definition has_this_π π := 
+match π with
+ | djs_π_main ϕ => has_this_ϕ ϕ
+end.
+
+(*
+   Detecting unbound this's in terms
+*)
+Definition has_this T :=
+match T with
+ | djs_term_λ  λ  => has_this_λ λ
+ | djs_term_λε λε => has_this_λε λε
+ | djs_term_ε  ε  => has_this_ε  ε
+ | djs_term_s  s  => has_this_stat s
+ | djs_term_ϕ  ϕ  => has_this_ϕ ϕ
+ | djs_term_δε δε => has_this_δε δε
+ | djs_term_π  π  => has_this_π π
+ | djs_interm  ι   => False
+end.
+
+(*
+   Detecting unbound this's in lists of terms 
+*)
+Definition has_this_list lT :=
+  ((fix has_this_lT lT : Prop :=
+      match lT with 
+        | nil => False
+        | T :: lT => has_this T \/ has_this_lT lT
+      end) lT).
+
+(* 
+   The procedure to detect this in a term is decidable 
+*)
+Lemma has_this_dec : forall T, {has_this T} + {~ has_this T}.
+Proof.
+  assert (Gλ : forall λ, (forall y, djs_size_term y < djs_size_term λ -> 
+                 {has_this y} + {~ has_this y}) -> {has_this λ} + {~ has_this λ}).
+  {
+    introv IH; destruct λ as [η | σ | β | lε | ρ]; try solve [simpls*].
+    + destruct lε as [ | ε lε]; jauto.
+      lets Hsize : djs_size_term_positive ε. 
+      destruct (IH ε) as [Hε | Hε]; try solve [simpls*; rew_length; nat_math].       
+      destruct (IH (djs_α lε)) as [Hlε | Hlε]; simpls; intuition.
+      
+    + destruct ρ as [ | (x & ε) ρ]; jauto.
+      lets Hsize : djs_size_term_positive ε. 
+      destruct (IH ε) as [Hε | Hε]; try solve [simpls*; rew_length; nat_math].       
+      destruct (IH (djs_ο ρ)) as [Hρ | Hρ]; simpls; intuition.
+  }
+
+   assert (Gλε : forall λε, (forall y, djs_size_term y < djs_size_term λε -> 
+                   {has_this y} + {~ has_this y}) -> {has_this λε} + {~ has_this λε}).
+  {
+    introv IH; destruct λε as [x | ε x | ε n | ε1 ε2 n | ε1 ε2 ].
+    + simpls; apply string_dec.
+    + apply (IH ε). simpls; nat_math.
+    + apply (IH ε). simpls; nat_math.
+    + destruct (IH ε1); simpls; [nat_math | intuition | ].
+      destruct (IH ε2); simpls; [nat_math | intuition | intuition ].
+    + destruct (IH ε1); simpls; [nat_math | intuition | ].
+      destruct (IH ε2); simpls; [nat_math | intuition | intuition ].
+  }
+
+   assert (Gε : forall ε, (forall y, djs_size_term y < djs_size_term ε -> 
+                 {has_this y} + {~ has_this y}) -> {has_this ε} + {~ has_this ε}).
+  {
+    introv IH; destruct ε as [ | | λε ε | unop ε | binop ε1 ε2 | ϕ lε | ε1 ε2 ]; try solve [simpls*; intuition]. 
+    + destruct (IH λε); simpls; [nat_math | intuition | ]. 
+      destruct (IH ε); simpls; [nat_math | intuition | intuition ].
+    + apply (IH ε). simpls; nat_math.
+    + destruct (IH ε1); simpls; [nat_math | intuition | ].
+      destruct (IH ε2); simpls; [nat_math | intuition | intuition ].
+    + destruct (IH ϕ) as [Hϕ | Hϕ]; [simpls; nat_math | simpls; intuition | ].
+      destruct lε as [ | ε lε]; [simpls* | ].
+      destruct (IH ε) as [Hε | Hε]; [ simpls; nat_math |  simpls; intuition | ].
+      lets Hsize : djs_size_term_positive ε.
+      destruct (IH (djs_ε_func ϕ lε)) as [Hlε | ]; simpls; [nat_math | intuition | intuition].
+    + destruct (IH ε1); simpls; [nat_math | intuition | ].
+      destruct (IH ε2); simpls; [nat_math | intuition | intuition ].
+  }
+
+  assert (Gs : forall s, (forall y, djs_size_term y < djs_size_term s -> 
+                 {has_this y} + {~ has_this y}) -> {has_this s} + {~ has_this s}).
+  {
+    introv IH; destruct s as [ | ε s | ε s1 s2 | ε s | ls ]; try solve [simpls*; intuition]. 
+    + destruct (IH ε); simpls; [nat_math | intuition | ]. 
+      destruct (IH s); simpls; [nat_math | |]; intuition.
+    + destruct (IH ε); simpls; [nat_math | intuition | ]. 
+      destruct (IH s1); simpls; [nat_math | intuition | ].
+      destruct (IH s2); simpls; [nat_math | |]; intuition.
+    + destruct (IH ε); simpls; [nat_math | intuition | ]. 
+      destruct (IH s); simpls; [nat_math | |]; intuition.
+    + destruct ls as [ | s ls]; simpls*.
+      lets Hsize : djs_size_term_positive s.
+      destruct (IH s); simpls; [nat_math | intuition | ]. 
+      destruct (IH (djs_stat_seq ls)); [simpls; nat_math | left | right];      
+      simpls; intuition.
+  }
+
+  assert (Gϕ : forall ϕ, (forall y, djs_size_term y < djs_size_term ϕ -> 
+                 {has_this y} + {~ has_this y}) -> {has_this ϕ} + {~ has_this ϕ}).
+  {
+    introv IH; destruct ϕ as [lx lyδε s ε].
+    lets Hs : (IH s). lets Hε : (IH ε).
+    destruct lx. simpls.
+    destruct Hs; destruct Hε; try solve [simpls; nat_math]; try solve [intuition].
+
+    cut ({(fix has_this_lvδε (lvδε : list (var * djs_δε)) : Prop :=
+             match lvδε with
+               | nil => False
+               | (_, δε) :: lvδε0 => has_this_δε δε \/ has_this_lvδε lvδε0
+             end) lyδε} + 
+         {~ (fix has_this_lvδε (lvδε : list (var * djs_δε)) : Prop :=
+               match lvδε with
+                 | nil => False
+                 | (_, δε) :: lvδε0 => has_this_δε δε \/ has_this_lvδε lvδε0
+               end) lyδε}).
+    introv Hyp; destruct (rm Hyp); intuition.
+    {
+      assert (Hm : forall x δε, Mem (x, δε) lyδε -> {has_this δε} + {~ has_this δε}).
+      {
+        introv Hm. apply IH.
+        cut (djs_size_term δε < S ((fix djs_size_lvδε (lvδε : list (var * djs_δε)) : nat :=
+                                      match lvδε with
+                                        | nil => 1
+                                        | (_, δε0) :: lvδε0 => (djs_size_δε δε0 + djs_size_lvδε lvδε0)%nat
+                                      end) lyδε)); [nat_math | ].
+
+
+        clear - Hm. gen x δε. inductions lyδε; introv Hm; inverts Hm as Hm. 
+        simpls; nat_math. specializes IHlyδε Hm. destruct a; nat_math.
+      }
+
+      clear - Hm. gen Hm. inductions lyδε; intros; [intuition | ].
+      destruct a as (xa & δεa).
+
+      destruct (Hm xa δεa); auto. constructor.
+      destruct IHlyδε; try solve [intuition]. 
+      introv Hm'; eapply Hm. constructor*. 
+    }
+    
+    destruct p as (x & τ).
+    simpls; cases_if*.
+    destruct Hs; destruct Hε; try solve [simpls; nat_math]; try solve [intuition].
+    destruct lyδε as [ | (y & δε) lyδε]. intuition.
+    destruct (IH δε). simpls; nat_math. intuition.
+    destruct (IH (djs_ϕ_main ((x, τ) :: lx) lyδε s ε)); [ | left | right].
+    lets Hsize : djs_size_term_positive δε. simpls; nat_math.
+      left. right. simpl in h; cases_if*.
+      rew_logic. repeat splits*. simpl in n2. cases_if*.
+      rewrite decide_spec in H. apply isTrue_true in e. unfolds var; false*. 
+  }
+
+  induction T using (measure_induction_type djs_size_term).
+  destruct T as [λ | λε | ε | s | ϕ | δε | π | ι]; jauto.
+  destruct δε as [ε | ϕ]; simpls; intuition.
+  destruct π as [ϕ]; simpls; intuition.
+ Qed.
+
+(* 
+   The procedure to detect this in a list of terms is decidable 
+*)
+Lemma has_this_list_dec : forall lT, {has_this_list lT} + {~ has_this_list lT}.
+Proof.
+  inductions lT; simpls*.
+  destruct (has_this_dec a) as [Ha | Ha]; intuition.
+Qed.
+
+End has_this. *)
+
+(* ********************************************************** *)
+(** * Unicity of types 
+
+Lemma djs_unicity_of_types_λ : 
+  forall λ Γ τm1 τm2 
+         (IH : forall T : djs_term,
+                 lt (djs_size_term T) (djs_size_term λ) ->
+                  forall Γ (τm1 τm2 : type), Γ |- T ∷ τm1 -> Γ |- T ∷ τm2 -> τm1 = τm2),
+    Γ |- λ ∷ τm1 -> Γ |- λ ∷ τm2 -> τm1 = τm2.
+Proof.
+  introv IH HD1 HD2; destruct λ; inverts HD1; inverts~ HD2.
+  
+  + lets Hτ : IH H0 H1. simpls; nat_math. inverts~ Hτ.
+  + lets Hτ : IH H0 H4. simpls; nat_math. inverts~ Hτ.
+    lets Hτ : IH H2 H6. lets Hsize : djs_size_term_positive ε1. 
+    simpls; rew_length; nat_math. inverts~ Hτ.
+  + lets Hτ : IH H1 H6. simpls; nat_math. inverts~ Hτ.
+    lets Hτ : IH H3 H8. lets Hsize : djs_size_term_positive ε. 
+    simpls; rew_length; nat_math. inverts~ Hτ.
+Qed.
+
+Lemma djs_unicity_of_types_λε : 
+  forall λε Γ τm1 τm2 
+         (IH : forall T : djs_term,
+                 lt (djs_size_term T) (djs_size_term λε) ->
+                  forall Γ (τm1 τm2 : type), Γ |- T ∷ τm1 -> Γ |- T ∷ τm2 -> τm1 = τm2),
+    Γ |- λε ∷ τm1 -> Γ |- λε ∷ τm2 -> τm1 = τm2.
+Proof.
+  introv IH HD1 HD2; destruct λε. 
+
+  + clear IH. inductions Γ. inverts HD1.
+    inversion HD1; inversion HD2; substs*.
+    - inverts H4. rewrite H3 in H8. inverts~ H8.
+    - inverts H4. false. apply H7. clear - H3.
+      gen v τ. inductions τρ0; introv HΦ; simpls; tryfalse.
+      destruct a. cases_if*; subst lx; rewrite (split_combine_fs τρ0).
+      * rewrite combine_split; [ | rewrite split_length_l; rewrite~ split_length_r]. 
+        simpls. inverts e. constructor.
+      * rewrite combine_split; [ | rewrite split_length_l; rewrite~ split_length_r]. 
+        simpls. constructor. jauto.
+    - inverts H5. false. apply H2. clear - H9.
+      gen v τ0. inductions τρ; introv HΦ; simpls.
+      * inverts HΦ.
+      * destruct a. cases_if*; subst lx; rewrite (split_combine_fs τρ).
+          rewrite combine_split; [ | rewrite split_length_l; rewrite~ split_length_r]. 
+          simpls. inverts e. constructor.
+          rewrite combine_split; [ | rewrite split_length_l; rewrite~ split_length_r]. 
+          simpls. constructor. jauto.
+
+  + inversion HD1; inversion HD2; substs.
+    specializes IH H2 H8. simpls; nat_math.
+    inverts IH. rewrite H10 in H4. inverts~ H4.
+
+  + inversion HD1; inversion HD2; substs.
+    specializes IH H2 H8. simpls; nat_math.
+    inverts~ IH. 
+
+  + inversion HD1; inversion HD2; substs.
+    specializes IH H2 H11. simpls; nat_math.
+    inverts~ IH. 
+
+  + inversion HD1; inversion HD2; substs.
+    specializes IH H2 H8. simpls; nat_math.
+    inverts~ IH. 
+Qed.
+
+Lemma djs_unicity_of_types_ε : 
+  forall ε Γ τm1 τm2 
+         (IH : forall T : djs_term,
+                 lt (djs_size_term T) (djs_size_term ε) ->
+                  forall Γ (τm1 τm2 : type), Γ |- T ∷ τm1 -> Γ |- T ∷ τm2 -> τm1 = τm2),
+    Γ |- ε ∷ τm1 -> Γ |- ε ∷ τm2 -> τm1 = τm2.
+Proof.
+  introv IH HD1 HD2; destruct ε; inversion HD1; inversion HD2; substs*;
+  try solve [tryfalse; clear HD1 HD2; eapply IH; try eassumption; simpls; nat_math].
+
+  + inverts H5. inverts H2.
+  + inverts H11. inverts H2.
+  + specializes IH H1 H8. simpls; nat_math. inverts~ IH.
+Qed.  
+
+Lemma djs_unicity_of_types_ϕ : 
+  forall ϕ Γ τm1 τm2 
+         (IH : forall T : djs_term,
+                 lt (djs_size_term T) (djs_size_term ϕ) ->
+                  forall Γ (τm1 τm2 : type), Γ |- T ∷ τm1 -> Γ |- T ∷ τm2 -> τm1 = τm2),
+    Γ |- ϕ ∷ τm1 -> Γ |- ϕ ∷ τm2 -> τm1 = τm2.
+Proof.
+  introv IH HD1 HD2; inversion HD1; inversion HD2; substs.
+
+  + symmetry in H6; inverts H6.
+    subst lx ly lτ lδε lx0 ly0 lτ0 lδε0. subst τρx0 τρy0.
+    clear - IH H4 H11; rename ls0 into ls; rename ε0 into ε.
+
+    remember nil as τρ. clear Heqτρ.
+    gen Γ τρx. inductions τρy; introv HD1 IH HD2.
+
+    - inverts HD1; inverts HD2.
+      cut (τr = τr0); try congruence.
+      specializes IH H6 H8; [simpls; nat_math | inverts~ IH].
+
+    - destruct a as (y & δε). inverts HD1; inverts* HD2.
+      eapply IHτρy; try eassumption. 
+      introv Hs HD1 HD2. eapply IH; try eassumption.
+      simpls; nat_math.
+      cut (τ = τ0); try congruence.
+      specializes IH H2 H3. simpls; nat_math. inverts~ IH.
+
+  + symmetry in H6; inverts H6.
+    subst lx ly lτ lδε lx0 ly0 lτ0 lδε0. subst τρx0 τρy0.
+    false*.
+
+  + symmetry in H8; inverts H8.
+    subst lx ly lτ lδε lx0 ly0 lτ0 lδε0. subst τρx0 τρy0.
+    false*.
+
+  + symmetry in H8; inverts H8.
+    subst lx ly lτ lδε lx0 ly0 lτ0 lδε0. subst τρx0 τρy0.
+    clear - IH H6 H15. admit.
+Qed.
+
+Theorem djs_unicity_of_types : 
+  forall T Γ τm1 τm2, 
+    Γ |- T ∷ τm1 -> Γ |- T ∷ τm2 -> τm1 = τm2.
+Proof.
+  induction T using (measure_induction djs_size_term).
+  destruct T as [λ | λε | ε | s | ϕ | δε | π | ι]; introv HD1 HD2.
+
+  + eapply djs_unicity_of_types_λ; eassumption.
+  + eapply djs_unicity_of_types_λε; eassumption.
+  + eapply djs_unicity_of_types_ε; eassumption.
+  + inverts HD1; inverts* HD2.
+  + eapply djs_unicity_of_types_ϕ; eassumption.
+  + inverts HD1; inverts* HD2; eapply H; try eassumption; simpls; nat_math.
+  + inverts HD1; inverts* HD2; eapply H; try eassumption; simpls; nat_math.
+  + inverts HD1; inverts* HD2. 
+Qed. *) *)
