coq/LibFsetExt.v
@@ -1,0 +1,399 @@
+Set Implicit Arguments.
+Require Import LibBag LibTactics LibFset LibReflect LibList LibLogic.
+
+(****** Basic Set Properties ******)
+
+Section Basic.
+Variables A : Type.
+Implicit Types E F: fset A.
+Implicit Types x y : A.
+
+
+Lemma in_and_notin: forall E x y, 
+  x \in E -> y \notin E -> x <> y.
+Proof.
+  introv H1 H2 H3. rewrite H3 in H1. false.
+Qed.
+
+(*This theorem its declared on LibFset but not recognized here*)
+(*Added the other implication making it an iff*)
+Axiom fset_extens_iff : forall E F,
+  (forall x, x \in E = x \in F) <-> E = F.
+
+Lemma fset_neq: forall E F,
+  (exists x, x \in E /\ x \notin E \n F) -> E <> F.
+Proof.
+  introv H. destruct H as (x & Hin & Hni). introv H.
+  lets K: fset_extens_iff E F. destruct K as (_ & H0). specializes H0 H x.
+  apply Hni. rewrite in_inter. split~.
+    rewrite~ <- H0.
+Qed.
+
+Lemma empty_dec: forall E, 
+  E = \{} \/ E <> \{}.
+Proof.
+  intro. lets (l & Hl): (fset_finite E). cases l.
+    rewrite from_list_nil in Hl. left~.
+    rewrite from_list_cons in Hl. right. rewrite Hl.
+    introv H. rewrite <- fset_extens_iff in H. specializes H a.
+    rewrite in_empty in H. rewrite <- H.
+    rewrite in_union. left. rewrite~ in_singleton.
+Qed.
+
+Lemma singleton_absurd: forall x, 
+  \{x} <> \{}.
+Proof.
+  introv. apply fset_neq. exists x. split.
+    rewrite~ in_singleton.
+    unfolds. introv H. rewrite inter_empty_r in H. rewrite~ in_empty in H.
+Qed.
+
+End Basic.
+
+
+
+(****** Remove Properties ******)
+
+Section Remove.
+Variables A : Type. 
+Implicit Types E F G: fset A.
+Implicit Types x: A.
+
+
+Lemma notin_remove : forall E F x, 
+  x \notin E \- F -> x \notin E \/ x \in F.
+Proof.
+  introv H.
+  unfolds notin.
+  rewrite in_remove in H. 
+  rew_logic in H. unfolds notin. rew_logic~ in H.
+Qed.
+
+Lemma remove_while_notin: forall E x, 
+  x \notin E -> E \- \{x} = E.
+Proof.
+  introv H; apply fset_extens; unfold subset; introv H1.
+    rewrite in_remove in H1. destruct~ H1.
+    rewrite in_remove. split~. rewrite notin_singleton. applys* in_and_notin.
+Qed.
+
+Lemma remove_in_subsets: forall E F G, 
+  E \c F -> E \- G \c F \- G.
+Proof.
+  introv H.
+    unfolds subset. introv H1. rewrite in_remove. split.
+      apply H. rewrite in_remove in H1. apply H1.
+      rewrite in_remove in H1. apply H1.
+Qed.
+
+Lemma remove_comm: forall E F G, 
+  (E \- F) \- G = (E \- G) \- F.
+Proof.
+  introv. apply fset_extens; unfold subset; intro; rewrite_all in_remove; introv H; intuition.
+Qed.    
+
+Lemma remove_same: forall E, 
+  (E \- E) = \{}.
+Proof.
+  introv. apply fset_extens; unfold subset; intro; rewrite in_remove; introv H.
+    false H. apply H.
+    rewrite in_empty in H. false.
+Qed.
+
+Lemma remove_empty: forall E, 
+  E \- \{} = E.
+Proof.
+  introv. apply fset_extens; unfold subset; intro; rewrite in_remove; introv H.
+    apply H.
+    split~.
+      apply notin_empty.
+Qed.
+
+Lemma remove_from_empty: forall E, 
+  (\{} \- E) = \{}.
+Proof.
+  introv. apply fset_extens; unfold subset; intro; rewrite in_remove; introv H.
+    apply H.
+    split.
+      apply H.
+      rewrite in_empty in H. false.
+Qed.
+
+Lemma from_rem_to_union: forall E F x, Comparable A ->
+  x \in F -> E = F \- \{x} -> \{x} \u E = F.
+Proof.
+  introv Hcmp H1 H2; apply fset_extens; unfold subset; introv H3.
+    rewrite in_union in H3. destruct H3.
+      rewrite in_singleton in H. rewrite~ H.
+      rewrite H2 in H. rewrite* in_remove in H.
+    rewrite in_union. eapply fset_extens_iff in H2. erewrite H2.
+      rewrite in_remove. rewrite in_singleton. rewrite notin_singleton.
+      destruct Hcmp. specializes comparable x x0. destruct comparable as (b & dec).
+      destruct b.
+        apply eq_true_l in dec. rewrite istrue_isTrue in dec. subst. left~.
+        apply eq_false_l in dec. rewrite istrue_neg in dec. rewrite istrue_isTrue in dec. right~.
+Qed.
+
+Lemma rem_union_cancel: forall E x, Comparable A ->
+  x \in E -> E \- \{x} \u \{x} = E.
+Proof.
+  introv Hcmp H. apply fset_extens; unfold subset; intros y H'.
+    rewrite in_union in H'. destruct H'.
+      rewrite in_remove in H0. destruct~ H0.
+      rewrite in_singleton in H0. subst~.
+    rewrite in_union. destruct Hcmp. specializes comparable x y.
+      destruct comparable as (b & dec). destruct b.
+        apply eq_true_l in dec. rewrite istrue_isTrue in dec. subst.
+        right. rewrite~ in_singleton.
+        apply eq_false_l in dec. rewrite istrue_neg in dec. rewrite istrue_isTrue in dec.
+        left. rewrite in_remove. rewrite notin_singleton. split~.
+Qed.
+
+Lemma remove_union: forall E F G,
+  E \- (F \u G) = (E \- F) \- G.
+Proof.
+  introv.
+  apply fset_extens; unfold subset; intro; rewrite_all in_remove; introv H.
+    rewrite* notin_union in H.
+    rewrite* notin_union.
+Qed.
+ 
+Lemma remove_union_distr : forall E F G,
+  (E \- G) \u (F \- G) = (E \u F) \- G.
+Proof.
+  introv; apply fset_extens; introv Hin; 
+  rewrite in_union in *; rewrite in_remove in *; inverts Hin; intuition; 
+  try rewrite in_union in *; try rewrite in_remove in *; try inverts H; jauto.
+Qed.
+
+Lemma remove_union_comm : forall E F x,
+ x \notin F -> (E \- F) \u \{x} = (E \u \{x}) \- F.
+Proof.
+  introv Hnin; apply fset_extens; introv Hin;
+  rewrite in_remove in *; rewrite in_union in *; rewrite in_remove in *;
+  inverts Hin; jauto.
+  rewrite in_singleton in H; subst; splits~.
+    right; rewrites~ in_singleton.
+  inverts H; jauto.
+Qed.
+
+End Remove.
+
+
+
+(****** Union Properties ******)
+
+Section Union.
+Variables A : Type. 
+Implicit Types E F G: fset A.
+Implicit Types x y: A.
+
+
+Lemma union_already_in: forall E x,  
+  x \in E -> \{x} \u E = E.
+Proof.
+  introv H. apply fset_extens; unfold subset; intros y H'.
+    rewrite in_union in H'. destruct~ H'.
+      rewrite in_singleton in H0. subst~.
+    rewrite in_union. right~.
+Qed.
+
+Lemma union_empty: forall E F, 
+  E \u F = \{} -> E=\{} /\ F = \{}.
+Proof.
+  introv H. split.
+    rewrite <- H. apply fset_extens; unfolds; introv H0.
+      rewrite in_union. left~.
+      eapply fset_extens_iff in H. rewrite H in H0. false. rewrite~ in_empty in H0.
+    rewrite <- H. apply fset_extens; unfolds; introv H0.
+      rewrite in_union. right~.
+      eapply fset_extens_iff in H. rewrite H in H0. false. rewrite~ in_empty in H0.
+Qed.
+
+Lemma from_union_to_rem: forall E F x, 
+  x \notin E -> \{x} \u E = F -> E = F \- \{x}.
+Proof.
+  introv H1 H2; apply fset_extens; unfold subset; introv H3.
+    rewrite <- H2. rewrite union_comm. rewrite union_remove. rewrite in_union.
+      left. rewrite~ remove_while_notin.
+    rewrite <- H2 in H3. rewrite union_comm in H3. rewrite union_remove in H3.
+      rewrite in_union in H3. destruct H3. rewrite~ remove_while_notin in H.
+      rewrite remove_same in H. rewrite* in_empty in H.
+Qed.
+
+Lemma union_subset: forall E F G, 
+  (E \u F) \c G -> E \c G.
+Proof.
+  unfold subset; introv H Hin.
+    apply H. rewrite in_union. left~.
+Qed.
+
+Lemma union_inv: forall E x y, 
+  \{x} \u E = \{y} -> x = y.
+Proof.
+  introv H.
+  lets H': fset_extens_iff. specializes H' A  (\{ x} \u E) (\{ y}).
+  destruct H'. specializes H1 H x. rewrite in_union in H1.
+  rewrite_all in_singleton in H1. rewrite <- H1.
+  left~.
+Qed.
+
+Lemma singleton_union: forall E F x, 
+  \{x} = E \u F -> x \in E \/ x \in F.
+Proof.
+  introv H.
+  lets H': fset_extens_iff. specializes H' A  \{ x} (E \u F).
+  destruct H'. specializes H1 H x. rewrite in_singleton in H1.
+  assert (x \in E \u F). rewrite~ <- H1. clear H1.
+  rewrite~ in_union in H2.
+Qed.
+
+Lemma union_not_empty: forall E F, 
+  E \u F <> \{} <-> E <> \{} \/ F <> \{}.
+Proof.
+  split. introv H.
+  destruct (empty_dec F).
+    left. rewrite <- (union_empty_r E). rewrite <- H0 at 1. assumption.
+    right~.
+  introv H1 H2. apply union_empty in H2. destruct H2 as (H2 & H3).
+  destruct H1 ; apply~ H.
+Qed.
+
+End Union.
+
+
+(****** Inter Properties ******)
+
+Section Inter.
+Variables A : Type. 
+Implicit Types E F G: fset A.
+
+Lemma inter_union: forall E F G,
+  (E \u F) \n G = \{} -> E \n G = \{} /\ F \n G = \{}.
+Proof.
+  introv H. split; apply fset_extens; rewrite <- fset_extens_iff in H; unfolds subset;
+  introv H1; specializes H x; rewrite in_inter in *.
+    rewrite <- H. rewrite in_union. split*.
+    rewrite in_empty in H1. false.
+    rewrite <- H. rewrite in_union. split*.
+    rewrite in_empty in H1. false.
+Qed.
+
+Lemma inter_remove: forall E F, (E \- F) \n F = \{}.
+Proof.
+  introv. apply fset_extens; unfolds subset; introv H;
+  rewrite in_inter in *; rewrite in_remove in *.
+    false H. apply H.
+    rewrite in_empty in H. false.
+Qed.
+
+Lemma inter_not_empty_exists : forall E F,
+  E \n F <> \{} -> exists x, x \in E \n F.
+Proof.
+  introv Hneq.
+  elim (classic (exists x, x \in E \n F)); introv Hnex; jauto.
+  false; apply Hneq.
+  apply fset_extens; introv Hin.
+  rewrite in_empty; rewrite* not_exists in Hnex.
+  rewrite* in_empty in Hin.
+Qed.
+
+Lemma inter_empty_subset : forall E1 E2 F1 F2, 
+  E1 \n E2 = \{} -> F1 \c E1 -> F2 \c E2 -> F1 \n F2 = \{}.
+Proof.
+  introv Hie Hs1 Hs2.
+    rewrite <- fset_extens_iff in Hie.
+    apply fset_extens; introv Hin.
+    rewrite in_inter in Hin; inverts Hin; apply Hs1 in H; apply Hs2 in H0.
+    rewrite <- (Hie x); rewrites* in_inter.
+    rewrite* in_empty in Hin.
+Qed.
+
+End Inter.
+
+(****** Subset Properties ******)
+
+Section Subset.
+Variables A : Type. 
+Implicit Types E F: fset A.
+Implicit Types x: A.
+
+
+Lemma fset_eq_sub: forall E F, 
+  E = F -> E \c F.
+Proof.
+  introv H.
+  rewrite H.
+  apply subset_refl.
+Qed.
+
+Lemma subset_of_empty: forall E, 
+  E \c \{} -> E = \{}.
+Proof.
+  introv H. apply fset_extens; unfolds subset; introv H1.
+    specializes~ H H1.
+    rewrite in_empty in H1. false.
+Qed.
+
+Lemma subset_union_r: forall E F x, 
+  x \notin E -> E \c (\{x} \u F) = E \c F.
+Proof.
+  introv H. unfolds subset. rew_logic. split; introv H1 H2.
+    specializes H1 x0 H2. rewrite in_union in H1. destruct~ H1.
+      rewrite in_singleton in H0. subst. false~ H.
+    specializes H1 x0 H2. rewrite~ in_union.
+Qed.
+
+
+End Subset.
+
+
+
+(****** From List Properties ******)
+
+Section FromList.
+Variables A : Type. 
+Implicit Types E F : fset A.
+Implicit Types l : list A.
+Implicit Types x : A.
+
+
+Lemma from_list_notin : forall l x, 
+  ~Mem x l -> x \notin from_list l.
+Proof.
+  induction l; introv Hnm.
+    rewrite from_list_nil. apply notin_empty.
+    rewrite from_list_cons. rewrite notin_union. split.
+      unfold notin. introv H. apply Hnm. rewrite in_singleton in H. rewrite H. apply Mem_here.
+      apply IHl. introv H. apply Hnm. constructor~.
+Qed.
+
+(*This theorem its declared on LibFset but not recognized here*)
+
+Lemma from_list_spec : forall x l,
+  x \in from_list l = Mem x l.
+Proof.
+  unfold from_list. induction l; rew_list.
+  rewrite in_empty. rewrite~ Mem_nil_eq. 
+  rewrite in_union, in_singleton. rewrite~ Mem_cons_eq. congruence.
+Qed.
+
+Lemma from_list_base: forall l, 
+  from_list l = \{} -> l = nil.
+Proof.
+  introv H. induction~ l.
+    rewrite from_list_cons in H. apply union_empty in H. false.
+    destruct H. eapply fset_extens_iff in H. rewrite in_singleton in H.
+    rewrite in_empty in H. rewrite~ <- H.
+Qed.
+
+Lemma from_list_app : forall l1 l2,
+  from_list (l1 ++ l2) = from_list l1 \u from_list l2.
+Proof.
+  introv; apply fset_extens; introv Hin; rewrite in_union in *; 
+    repeat rewrite from_list_spec in *; rewrite Mem_app_or_eq in *; auto.   
+Qed.
+
+End FromList.
+
+
